full_message vlsm is equal to validating projection (#38)
* Refactorings

* full_message vlsm is equal to validating projection

VLSM/ByzantineFaults.v
@@ -1,4 +1,4 @@
-Require Import FinFun.
+Require Import FinFun Streams.
 (* Section 4: Byzantine fault tolerance analysis *)
 From Casper   
 Require Import Lib.Preamble VLSM.Common VLSM.Composition.
@@ -17,7 +17,7 @@ Context
     (X := indexed_vlsm_constrained i0 IM constraint)
     .
 
-Definition validating_received_messages
+Definition validating_messages
     (i : index)
     :=
     forall (si : @state _ (IT i)) (mi : message) (li : @label _ (IT i)),
@@ -31,18 +31,18 @@ Definition validating_received_messages
         -> ~ @valid _ _ _ (IM i) li (si, Some mi)
             .
 
-Definition validating_messages
+Definition validating_condition
     (i : index)
     :=
     forall (li : @label _ (IT i)) (siomi : @state _ (IT i) * option message),
         @valid _ _ _ (IM i) li siomi ->
-        composite_protocol_valid i0 IM constraint i li siomi.
+        projection_valid i0 IM constraint i li siomi.
 
 Lemma validating_messages_received
     (i : index)
-    : validating_messages i -> validating_received_messages i.
+    : validating_condition i -> validating_messages i.
 Proof.
-    unfold validating_messages. unfold validating_received_messages. intros.
+    unfold validating_condition. unfold validating_messages. intros.
     intro Hvalid. apply H0. clear H0.
     specialize (H li (si, Some mi) Hvalid). clear Hvalid.
     destruct H as [ps [opm [Hsi [Hmi Hvalid]]]].
@@ -74,10 +74,10 @@ Definition validating_transitions
 
 Lemma validating_messages_transitions
     (i : index)
-    : validating_messages i -> validating_transitions i.
+    : validating_condition i -> validating_transitions i.
 Proof.
-    unfold validating_messages. unfold validating_transitions. 
-    unfold composite_protocol_valid. unfold verbose_valid_protocol_transition.
+    unfold validating_condition. unfold validating_transitions. 
+    unfold projection_valid. unfold verbose_valid_protocol_transition.
     simpl. intros.
     specialize (H li (si, omi) H0). clear H0. simpl in H.
     destruct H as [ps [opm [Hsi [Homi Hvalid]]]].
@@ -101,9 +101,9 @@ Qed.
     
 Lemma validating_transitions_messages
     (i : index)
-    : validating_transitions i -> validating_messages i.
+    : validating_transitions i -> validating_condition i.
 Proof.
-    unfold validating_messages. unfold validating_transitions. intros.
+    unfold validating_condition. unfold validating_transitions. intros.
     destruct siomi as [si omi].
     specialize (H si omi li H0); clear H0.
     destruct H as [s [s' [om' [Hsi [Hps [Hopm [Hvalid Htransition]]]]]]].
@@ -116,3 +116,134 @@ Proof.
       repeat (split; try assumption).
 Qed.
 
+Section message_full_validating_proj.
+    Context
+        (i : index)
+        (Hvalidating : validating_condition i)
+        (Proj := indexed_vlsm_constrained_projection i0 IM constraint i)
+        (Full := message_full_vlsm (IM i))
+        .
+
+    Lemma validating_proj_protocol_message
+        (m : message)
+        (li : label)
+        (si : state)
+        (Hvalid_m : @valid _ _ _ (IM i) li (si, Some m))
+        : protocol_message_prop Proj m
+        .
+    Proof.
+        apply Hvalidating in Hvalid_m.
+        destruct Hvalid_m as [ps [opm [Hsi [Hm Hvalid]]]].
+        destruct opm as [[m' Hpm]|]; try inversion Hm; clear Hm; subst.
+        apply protocol_message_projection. assumption.
+    Qed.
+
+
+
+    Lemma _message_full_validating_proj_protocol_state
+        (som : state * option message)
+        (Hps : protocol_prop Full som)
+        : protocol_state_prop Proj (fst som).
+    Proof.
+        induction Hps.
+        - exists None. apply (protocol_initial_state Proj is).
+        - exists None. apply (protocol_initial_state Proj (@VLSM.Common.s0 _ _ (IS i))).
+        - destruct
+            (@transition message (IT i) (@message_full_vlsm_sig message (IT i) (IS i) (IM i)) Full l
+                (@pair (@state message (IT i)) (option message) s om)) as [s' om'] eqn:Ht.
+          exists om'. simpl. rewrite <- Ht.
+          clear IHHps2. simpl in IHHps1. clear Hps1 Hps2 _s _om.
+          destruct IHHps1 as [_om Hps].
+          destruct om as [m|].
+          + specialize (validating_proj_protocol_message m l s Hv); intros [_s Hpm].
+            apply (protocol_generated Proj) with _om _s; try assumption.
+            apply Hvalidating. assumption.
+          + apply (protocol_generated Proj) with _om (proj1_sig s0); try assumption.
+            * apply (protocol_initial_state Proj s0).
+            * apply Hvalidating. assumption.
+    Qed.
+
+    Lemma message_full_validating_proj_protocol_state
+        (s : state)
+        (om : option message)
+        (Hps : protocol_prop Full (s,om))
+        : protocol_state_prop Proj s.
+    Proof.
+        remember (s, om) as som. 
+        assert (Hs : s = fst som) by (subst; reflexivity).
+        rewrite Hs. apply _message_full_validating_proj_protocol_state.
+        assumption.
+    Qed.
+
+    Lemma message_full_validating_proj_verbose_valid_protocol_transition
+        (l : label)
+        (is os : state)
+        (iom oom : option message)
+        (Ht : verbose_valid_protocol_transition Full l is os iom oom)
+        : verbose_valid_protocol_transition Proj l is os iom oom
+        .
+    Proof.
+        destruct Ht as [[_om Hps] [[_s Hpm] [Hv Ht]]].
+        repeat (split; try assumption).
+        - apply message_full_validating_proj_protocol_state with _om.
+          assumption.
+        - destruct iom as [im|].
+          + apply validating_proj_protocol_message with l is. assumption.
+          + exists (proj1_sig s0). apply (protocol_initial_state Proj s0).
+        - apply Hvalidating. assumption.
+    Qed.
+
+    Lemma message_full_validating_proj_finite_ptrace
+        (s : state)
+        (ls : list in_state_out)
+        (Hpxt : finite_ptrace_from Full s ls)
+        : finite_ptrace_from Proj s ls
+        .
+    Proof.
+        induction Hpxt.
+        - constructor.
+          destruct H as [m H].
+          apply message_full_validating_proj_protocol_state with m. assumption.
+        - constructor; try assumption.
+          apply message_full_validating_proj_verbose_valid_protocol_transition.
+          assumption.
+    Qed.
+
+    Lemma message_full_validating_proj_infinite_ptrace
+        (s : state)
+        (ls : Stream in_state_out)
+        (Hpxt : infinite_ptrace_from Full s ls)
+        : infinite_ptrace_from Proj s ls
+        .
+    Proof.
+        generalize dependent ls. generalize dependent s.
+        cofix H.
+        intros s [[l input destination output] ls] Hx.
+        inversion Hx; subst.
+        specialize (H destination ls H3).
+        constructor; try assumption.
+        apply message_full_validating_proj_verbose_valid_protocol_transition.
+        assumption.
+    Qed.
+
+    Lemma message_full_validating_proj_incl
+        : VLSM_incl Full Proj
+        .
+    Proof.
+        intros [s ls| s ss]; simpl; intros [Hxt Hinit].  
+        - apply message_full_validating_proj_finite_ptrace in Hxt.
+          split; try assumption.
+        - apply message_full_validating_proj_infinite_ptrace in Hxt.
+          split; try assumption.
+    Qed.
+
+    Lemma message_full_validating_proj_eq
+        : VLSM_eq Full Proj
+        .
+    Proof.
+        split.
+        - apply message_full_validating_proj_incl.
+        - apply proj_message_full_incl.
+    Qed.
+
+End message_full_validating_proj.
