VLSM/Common.v
@@ -20,1222 +20,1396 @@ Require Import Lib.Preamble Lib.ListExtras.
     ; l0 : label
     }.
 
-    Class VLSM {message : Type} {vtype : VLSM_type message} (lsm : LSM_sig vtype) :=
-      { transition : label -> state * option message -> state * option message
-      ; valid : label -> state * option message -> Prop
-      }.
+  Class VLSM {message : Type} {vtype : VLSM_type message} (lsm : LSM_sig vtype) :=
+    { transition : label -> state * option message -> state * option message
+    ; valid : label -> state * option message -> Prop
+    }.
 
-    Definition sign
+  Definition sign
+    {message : Type}
+    {vtype : VLSM_type message}
+    {Sig : LSM_sig vtype}
+    (vlsm : VLSM Sig)
+    := Sig.
+
+  Definition type
+    {message : Type}
+    {vtype : VLSM_type message}
+    {Sig : LSM_sig vtype}
+    (vlsm : VLSM Sig)
+    := vtype.
+
+  Section VLSM.
+
+    Context
       {message : Type}
       {vtype : VLSM_type message}
       {Sig : LSM_sig vtype}
-      (vlsm : VLSM Sig)
-      := Sig.
+      (vlsm : VLSM Sig). 
 
-    Definition type
-      {message : Type}
-      {vtype : VLSM_type message}
-      {Sig : LSM_sig vtype}
-      (vlsm : VLSM Sig)
-      := vtype.
+  (* 2.2.2 VLSM protocol states and protocol messages *)
 
-    Section VLSM.
+  (* We choose here to use the second definition hinted at the end of Section 2.2.2,
+     i.e., we define states and messages together as a property over a product type.
+  *)
 
-      Context
-        {message : Type}
-        {vtype : VLSM_type message}
-        {Sig : LSM_sig vtype}
-        (vlsm : VLSM Sig). 
+    Inductive protocol_prop : state * option message -> Prop :=
+    | protocol_initial_state
+        (is : initial_state)
+        (s : state := proj1_sig is)
+      : protocol_prop (s, None)
+    | protocol_initial_message
+        (im : initial_message)
+        (s : state := proj1_sig s0)
+        (om : option message := Some (proj1_sig im))
+      : protocol_prop (s, om)
+    | protocol_generated
+        (l : label)
+        (s : state)
+        (_om : option message)
+        (Hps : protocol_prop (s, _om))
+        (_s : state)
+        (om : option message)
+        (Hpm : protocol_prop (_s, om))
+        (Hv : valid l (s, om))
+      : protocol_prop (transition l (s, om)).
 
-      (* 2.2.2 VLSM protocol states and protocol messages *)
+    Definition protocol_state_prop (s : state) :=
+      exists om : option message, protocol_prop (s, om).
 
-      (* We choose here to use the second definition hinted at the end of the 2.2.2 section, i.e., 
-we define states and messages together as a property over a product type. *)
+    Definition protocol_message_prop (m : message) :=
+      exists s : state, protocol_prop (s, (Some m)).
 
-      Inductive protocol_prop : state * option message -> Prop :=
-      | protocol_initial_state
-          (is : initial_state)
-          (s : state := proj1_sig is)
-        : protocol_prop (s, None)
-      | protocol_initial_message
-          (im : initial_message)
-          (s : state := proj1_sig s0)
-          (om : option message := Some (proj1_sig im))
-        : protocol_prop (s, om)
-      | protocol_generated
-          (l : label)
-          (s : state)
-          (_om : option message)
-          (Hps : protocol_prop (s, _om))
-          (_s : state)
-          (om : option message)
-          (Hpm : protocol_prop (_s, om))
-          (Hv : valid l (s, om))
-        : protocol_prop (transition l (s, om)).
+    Definition protocol_state : Type :=
+      { s : state | protocol_state_prop s }.
 
-      Definition protocol_state_prop (s : state) :=
-        exists om : option message, protocol_prop (s, om).
+    Definition protocol_message : Type :=
+      { m : message | protocol_message_prop m }.
+    
+    (* Restating validity and transition using protocol_state and protocol_messages. *)
 
-      Definition protocol_message_prop (m : message) :=
-        exists s : state, protocol_prop (s, (Some m)).
+    Definition protocol_valid
+               (l : label)
+               (ps_opm : protocol_state * option protocol_message)
+      : Prop :=
+      valid l (proj1_sig (fst ps_opm), option_map (@proj1_sig _ _) (snd ps_opm)).
 
-      Definition protocol_state : Type :=
-        { s : state | protocol_state_prop s }.
+    Definition protocol_transition
+               (l : label)
+               (ps_opm : protocol_state * option protocol_message)
+      : state * option message :=
+      transition l (proj1_sig (fst ps_opm), option_map (@proj1_sig _ _) (snd ps_opm)).
 
-      Definition protocol_message : Type :=
-        { m : message | protocol_message_prop m }.
-      
-      (* Restating validity and transition using protocol_state and protocol_messages. *)
+    Definition lift_option_proto_message 
+               (om : option message)
+               (_s : state)
+               (Hm : protocol_prop (_s, om))
+      : option protocol_message.
+      destruct om as [m|].
+      - apply Some. exists m. exists _s. assumption.
+      - exact None.
+    Defined.
 
-      Definition protocol_valid
-                 (l : label)
-                 (ps_opm : protocol_state * option protocol_message)
-        : Prop :=
-        valid l (proj1_sig (fst ps_opm), option_map (@proj1_sig _ _) (snd ps_opm)).
+    (* Protocol state characterization - similar to the definition in the report. *)
 
-      Definition protocol_transition
-                 (l : label)
-                 (ps_opm : protocol_state * option protocol_message)
-        : state * option message :=
-        transition l (proj1_sig (fst ps_opm), option_map (@proj1_sig _ _) (snd ps_opm)).
-
-      Definition lift_option_proto_message 
-                 (om : option message)
-                 (_s : state)
-                 (Hm : protocol_prop (_s, om))
-        : option protocol_message.
-        destruct om as [m|].
-        - apply Some. exists m. exists _s. assumption.
-        - exact None.
-      Defined.
-
-      (* Protocol state characterization - similar to the definition in the report. *)
-
-      Lemma protocol_state_prop_iff :
-        forall s' : state,
-          protocol_state_prop s'
-          <-> (exists is : initial_state, s' = proj1_sig is)
-            \/ exists (s : protocol_state) (l : label) (om : option protocol_message),
-              protocol_valid l (s, om)
-              /\ s' = fst (protocol_transition l (s, om)).
-      Proof.
-        intros; split.
-        - intro Hps'. destruct Hps' as [m' Hs].
-          inversion Hs; subst
-          ; try (left; exists is; reflexivity)
-          ; try (left; exists s0; reflexivity).
-          right. exists (exist _ s (ex_intro _ _ Hps)). exists l.
-          exists (lift_option_proto_message om _s Hpm).
-          unfold protocol_valid. unfold protocol_transition.
-          unfold lift_option_proto_message. 
-          destruct om as [m|]; simpl
-          ; simpl
-          ; rewrite H0
-          ; split
-          ; auto
-          .
-        - intros [[[s His] Heq] | [[s Hps] [l [om [Hv Ht]]]]]; subst.
-          + exists None. apply protocol_initial_state.
-          + exists (snd (protocol_transition l (exist (fun s1 : state => protocol_state_prop s1) s Hps, om))).
-            destruct Hps as [_om Hps].
-            specialize (protocol_generated l s _om Hps); intros Hps'.
-            unfold protocol_transition.
-            destruct om as [[m [_s Hpm]]|].
-            * specialize (Hps' _s (Some m) Hpm Hv). simpl.
-              destruct (transition l (s, Some m)) as [s' om'].
-              assumption.
-            * specialize (Hps' (proj1_sig s0) None (protocol_initial_state s0) Hv). simpl.
-              destruct (transition l (s, None)) as [s' om']. assumption.
-      Qed.
-
-      (* Protocol message characterization - similar to the definition in the report. *)
-
-      Lemma protocol_message_prop_iff :
-        forall m' : message,
-          protocol_message_prop m'
-          <-> (exists im : initial_message, m' = proj1_sig im)
-            \/ exists (s : protocol_state) (l : label) (om : option protocol_message),
-              protocol_valid l (s, om)
-              /\ Some m' = snd (protocol_transition l (s, om)).
-      Proof.
-        intros; split.
-        - intros [s' Hpm'].
-          inversion Hpm'; subst
-          ; try (left; exists im; reflexivity).
-          right. exists (exist _ s (ex_intro _ _ Hps)). exists l.
-          exists (lift_option_proto_message om _s Hpm).
-          unfold protocol_valid. unfold protocol_transition.
-          unfold lift_option_proto_message. 
-          destruct om as [m|]
-          ; simpl
-          ; rewrite H0
-          ; split
-          ; auto
-          .
-        - intros [[[m Him] Heq] | [[s Hps] [l [om [Hv Ht]]]]]; subst.
-          + exists (proj1_sig s0). apply protocol_initial_message.
-          + exists (fst (protocol_transition l (exist (fun s1 : state => protocol_state_prop s1) s Hps, om))).
-            destruct Hps as [_om Hps].
-            specialize (protocol_generated l s _om Hps); intros Hps'.
-            unfold protocol_transition.
-            destruct om as [[m [_s Hpm]]|]
-            ; specialize (Hps' _s (Some m) Hpm Hv) || specialize (Hps' (proj1_sig s0) None (protocol_initial_state s0) Hv)
-            ; simpl
-            ; unfold protocol_transition in Ht; simpl in Ht
-            ; destruct (transition l (s, Some m)) as [s' om'] || destruct (transition l (s, None)) as [s' om']
-            ; simpl in Ht; subst
-            ;  assumption
-            .
-      Qed.
-
-      Corollary protocol_state_destruct :
-        forall s' : protocol_state,
-          (exists is : initial_state, proj1_sig s' = proj1_sig is)
+    Lemma protocol_state_prop_iff :
+      forall s' : state,
+        protocol_state_prop s'
+        <-> (exists is : initial_state, s' = proj1_sig is)
           \/ exists (s : protocol_state) (l : label) (om : option protocol_message),
             protocol_valid l (s, om)
-            /\ proj1_sig s' = fst (protocol_transition l (s, om)).
-      Proof.
-        intros [s' Hps']. simpl. apply protocol_state_prop_iff. assumption.
-      Qed.
-
-      (* Induction principle for protocol states *)
-
-      Lemma protocol_state_ind
-        : forall (P : state -> Prop),
-          (forall is : initial_state, P (proj1_sig is)) ->
-          (forall (s : protocol_state) (Hind : P (proj1_sig s)) (l : label) (om : option protocol_message)
-             (Hv : protocol_valid l (s, om)),
-              P (fst (protocol_transition l (s, om)))) ->
-          (forall s : protocol_state, P (proj1_sig s)).
-      Proof.
-        intros P HIi HIt.
-        assert (Hind : forall som' : state * option message, protocol_prop som' -> P (fst som')).
-        { intros som' Hp.
-          induction Hp; try apply HIi.
-          specialize (HIt (exist _ s (ex_intro _ _ Hp1)) IHHp1 l (lift_option_proto_message om _s Hp2)).
-          unfold protocol_valid in HIt. 
-          unfold lift_option_proto_message in HIt. 
-          destruct om as [m|]
-          ; specialize (HIt Hv)
-          ; assumption.
-        }
-        intros [s' [om' Hps]]. simpl.
-        specialize (Hind (s', om') Hps). assumption.
-      Qed.
-
-      (* Section 2.2.3 Valid VLSM transitions, VLSM traces, and VLSM identity *)
-
-      (* Valid VLSM transitions *)
-
-      Definition verbose_valid_protocol_transition
-                 (l : label)
-                 (s s' : state)
-                 (om om' : option message)
-        := (exists (_om : option message), protocol_prop (s, _om))
-        /\ (exists (_s : state), protocol_prop (_s, om))
-        /\  valid l (s, om)
-        /\  transition l (s, om) = (s', om')
+            /\ s' = fst (protocol_transition l (s, om)).
+    Proof.
+      intros; split.
+      - intro Hps'. destruct Hps' as [m' Hs].
+        inversion Hs; subst
+        ; try (left; exists is; reflexivity)
+        ; try (left; exists s0; reflexivity).
+        right. exists (exist _ s (ex_intro _ _ Hps)). exists l.
+        exists (lift_option_proto_message om _s Hpm).
+        unfold protocol_valid. unfold protocol_transition.
+        unfold lift_option_proto_message. 
+        destruct om as [m|]; simpl
+        ; simpl
+        ; rewrite H0
+        ; split
+        ; auto
         .
+      - intros [[[s His] Heq] | [[s Hps] [l [om [Hv Ht]]]]]; subst.
+        + exists None. apply protocol_initial_state.
+        + exists (snd (protocol_transition l (exist (fun s1 : state => protocol_state_prop s1) s Hps, om))).
+          destruct Hps as [_om Hps].
+          specialize (protocol_generated l s _om Hps); intros Hps'.
+          unfold protocol_transition.
+          destruct om as [[m [_s Hpm]]|].
+          * specialize (Hps' _s (Some m) Hpm Hv). simpl.
+            destruct (transition l (s, Some m)) as [s' om'].
+            assumption.
+          * specialize (Hps' (proj1_sig s0) None (protocol_initial_state s0) Hv). simpl.
+            destruct (transition l (s, None)) as [s' om']. assumption.
+    Qed.
 
-      Lemma protocol_transition_origin
-            {l : label}
-            {s s' : state}
-            {om om' : option message}
-            (Ht : verbose_valid_protocol_transition l s s' om om')
-        : protocol_state_prop s
-      .
-      Proof.
-        destruct Ht as [[_om Hp] _]. exists _om. assumption.
-      Qed.
+    (* Protocol message characterization - similar to the definition in the report. *)
 
-      Lemma protocol_transition_destination
-            {l : label}
-            {s s' : state}
-            {om om' : option message}
-            (Ht : verbose_valid_protocol_transition l s s' om om')
-        : protocol_state_prop s'
-      .
-      Proof.
-        exists om'. 
-        destruct Ht as [[_om Hs] [[_s Hom] [Hv Ht]]].
-        rewrite <- Ht. apply protocol_generated with _om _s; assumption.
-      Qed.
-
-      Lemma protocol_transition_in
-            {l : label}
-            {s s' : state}
-            {m : message}
-            {om' : option message}
-            (Ht : verbose_valid_protocol_transition l s s' (Some m) om')
-        : protocol_message_prop m
-      .
-      Proof.
-        destruct Ht as [_ [[_s Hom] _]].
-        exists _s. assumption.
-      Qed.
-
-      Lemma protocol_prop_transition_in
-            {l : label}
-            {s s' : state}
-            {om om' : option message}
-            (Ht : verbose_valid_protocol_transition l s s' om om')
-        : exists _s, protocol_prop (_s, om).
-      Proof.
-        destruct om as [m|].
-        - apply protocol_transition_in in Ht.
-          inversion Ht. exists x. assumption.
-        - exists (proj1_sig s0). constructor.
-      Qed.
-
-      Lemma protocol_transition_out
-            {l : label}
-            {s s' : state}
-            {om : option message}
-            {m' : message}
-            (Ht : verbose_valid_protocol_transition l s s' om (Some m'))
-        : protocol_message_prop m'
-      .
-      Proof.
-        exists s'. 
-        destruct Ht as [[_om Hs] [[_s Hom] [Hv Ht]]].
-        rewrite <- Ht. apply protocol_generated with _om _s; assumption.
-      Qed.
-
-      Lemma protocol_transition_valid
-            {l : label}
-            {s s' : state}
-            {om om' : option message}
-            (Ht : verbose_valid_protocol_transition l s s' om om')
-        : valid l (s, om).
-      Proof.
-        destruct Ht as [_ [_ [Hv _]]].
-        assumption.
-      Qed.
-
-      Lemma protocol_transition_transition
-            {l : label}
-            {s s' : state}
-            {om om' : option message}
-            (Ht : verbose_valid_protocol_transition l s s' om om')
-          :  transition l (s, om) = (s', om')
+    Lemma protocol_message_prop_iff :
+      forall m' : message,
+        protocol_message_prop m'
+        <-> (exists im : initial_message, m' = proj1_sig im)
+          \/ exists (s : protocol_state) (l : label) (om : option protocol_message),
+            protocol_valid l (s, om)
+            /\ Some m' = snd (protocol_transition l (s, om)).
+    Proof.
+      intros; split.
+      - intros [s' Hpm'].
+        inversion Hpm'; subst
+        ; try (left; exists im; reflexivity).
+        right. exists (exist _ s (ex_intro _ _ Hps)). exists l.
+        exists (lift_option_proto_message om _s Hpm).
+        unfold protocol_valid. unfold protocol_transition.
+        unfold lift_option_proto_message. 
+        destruct om as [m|]
+        ; simpl
+        ; rewrite H0
+        ; split
+        ; auto
         .
-       Proof.
-        destruct Ht as [_ [_ [_ Ht]]]. assumption.
-       Qed.
+      - intros [[[m Him] Heq] | [[s Hps] [l [om [Hv Ht]]]]]; subst.
+        + exists (proj1_sig s0). apply protocol_initial_message.
+        + exists (fst (protocol_transition l (exist (fun s1 : state => protocol_state_prop s1) s Hps, om))).
+          destruct Hps as [_om Hps].
+          specialize (protocol_generated l s _om Hps); intros Hps'.
+          unfold protocol_transition.
+          destruct om as [[m [_s Hpm]]|]
+          ; specialize (Hps' _s (Some m) Hpm Hv) || specialize (Hps' (proj1_sig s0) None (protocol_initial_state s0) Hv)
+          ; simpl
+          ; unfold protocol_transition in Ht; simpl in Ht
+          ; destruct (transition l (s, Some m)) as [s' om'] || destruct (transition l (s, None)) as [s' om']
+          ; simpl in Ht; subst
+          ;  assumption
+          .
+    Qed.
+
+    Corollary protocol_state_destruct :
+      forall s' : protocol_state,
+        (exists is : initial_state, proj1_sig s' = proj1_sig is)
+        \/ exists (s : protocol_state) (l : label) (om : option protocol_message),
+          protocol_valid l (s, om)
+          /\ proj1_sig s' = fst (protocol_transition l (s, om)).
+    Proof.
+      intros [s' Hps']. simpl. apply protocol_state_prop_iff. assumption.
+    Qed.
+
+    (* Induction principle for protocol states *)
+
+    Lemma protocol_state_ind
+      : forall (P : state -> Prop),
+        (forall is : initial_state, P (proj1_sig is)) ->
+        (forall (s : protocol_state) (Hind : P (proj1_sig s)) (l : label) (om : option protocol_message)
+           (Hv : protocol_valid l (s, om)),
+            P (fst (protocol_transition l (s, om)))) ->
+        (forall s : protocol_state, P (proj1_sig s)).
+    Proof.
+      intros P HIi HIt.
+      assert (Hind : forall som' : state * option message, protocol_prop som' -> P (fst som')).
+      { intros som' Hp.
+        induction Hp; try apply HIi.
+        specialize (HIt (exist _ s (ex_intro _ _ Hp1)) IHHp1 l (lift_option_proto_message om _s Hp2)).
+        unfold protocol_valid in HIt. 
+        unfold lift_option_proto_message in HIt. 
+        destruct om as [m|]
+        ; specialize (HIt Hv)
+        ; assumption.
+      }
+      intros [s' [om' Hps]]. simpl.
+      specialize (Hind (s', om') Hps). assumption.
+    Qed.
+
+    (* Section 2.2.3 Valid VLSM transitions, VLSM traces, and VLSM identity *)
+
+    (* Valid VLSM transitions *)
+
+    Definition verbose_valid_protocol_transition
+               (l : label)
+               (s s' : state)
+               (om om' : option message)
+      := (exists (_om : option message), protocol_prop (s, _om))
+      /\ (exists (_s : state), protocol_prop (_s, om))
+      /\  valid l (s, om)
+      /\  transition l (s, om) = (s', om')
+      .
+
+    Lemma protocol_transition_origin
+          {l : label}
+          {s s' : state}
+          {om om' : option message}
+          (Ht : verbose_valid_protocol_transition l s s' om om')
+      : protocol_state_prop s
+    .
+    Proof.
+      destruct Ht as [[_om Hp] _]. exists _om. assumption.
+    Qed.
+
+    Lemma protocol_transition_destination
+          {l : label}
+          {s s' : state}
+          {om om' : option message}
+          (Ht : verbose_valid_protocol_transition l s s' om om')
+      : protocol_state_prop s'
+    .
+    Proof.
+      exists om'. 
+      destruct Ht as [[_om Hs] [[_s Hom] [Hv Ht]]].
+      rewrite <- Ht. apply protocol_generated with _om _s; assumption.
+    Qed.
+
+    Lemma protocol_transition_in
+          {l : label}
+          {s s' : state}
+          {m : message}
+          {om' : option message}
+          (Ht : verbose_valid_protocol_transition l s s' (Some m) om')
+      : protocol_message_prop m
+    .
+    Proof.
+      destruct Ht as [_ [[_s Hom] _]].
+      exists _s. assumption.
+    Qed.
+
+    Lemma protocol_prop_transition_in
+          {l : label}
+          {s s' : state}
+          {om om' : option message}
+          (Ht : verbose_valid_protocol_transition l s s' om om')
+      : exists _s, protocol_prop (_s, om).
+    Proof.
+      destruct om as [m|].
+      - apply protocol_transition_in in Ht.
+        inversion Ht. exists x. assumption.
+      - exists (proj1_sig s0). constructor.
+    Qed.
+
+    Lemma protocol_transition_out
+          {l : label}
+          {s s' : state}
+          {om : option message}
+          {m' : message}
+          (Ht : verbose_valid_protocol_transition l s s' om (Some m'))
+      : protocol_message_prop m'
+    .
+    Proof.
+      exists s'. 
+      destruct Ht as [[_om Hs] [[_s Hom] [Hv Ht]]].
+      rewrite <- Ht. apply protocol_generated with _om _s; assumption.
+    Qed.
+
+    Lemma protocol_transition_valid
+          {l : label}
+          {s s' : state}
+          {om om' : option message}
+          (Ht : verbose_valid_protocol_transition l s s' om om')
+      : valid l (s, om).
+    Proof.
+      destruct Ht as [_ [_ [Hv _]]].
+      assumption.
+    Qed.
+
+    Lemma protocol_transition_transition
+          {l : label}
+          {s s' : state}
+          {om om' : option message}
+          (Ht : verbose_valid_protocol_transition l s s' om om')
+        :  transition l (s, om) = (s', om')
+      .
+     Proof.
+      destruct Ht as [_ [_ [_ Ht]]]. assumption.
+     Qed.
 
 
-      (* Valid VLSM traces *) 
-      Record in_state_out :=
-        {   l : label
-            ;   input : option message
-            ;   destination : state
-            ;   output : option message
-        }.
+    (* Valid VLSM traces *) 
+    Record in_state_out :=
+      {   l : label
+          ;   input : option message
+          ;   destination : state
+          ;   output : option message
+      }.
 
-      (* A finite protocol trace originating in a given state *)
-      
-      Inductive finite_ptrace_from : state -> list in_state_out -> Prop :=
-      | finite_ptrace_empty : forall (s : state), protocol_state_prop s -> finite_ptrace_from s []
-      | finite_ptrace_extend : forall  (s : state) (tl : list in_state_out),
-          finite_ptrace_from s tl ->  
-          forall (s' : state) (iom oom : option message) (l : label),
-            verbose_valid_protocol_transition l s' s iom oom ->
-            finite_ptrace_from  s' ({| l := l; input := iom; destination := s; output := oom |} :: tl).
+    (* A finite protocol trace originating in a given state *)
+    
+    Inductive finite_ptrace_from : state -> list in_state_out -> Prop :=
+    | finite_ptrace_empty : forall (s : state), protocol_state_prop s -> finite_ptrace_from s []
+    | finite_ptrace_extend : forall  (s : state) (tl : list in_state_out),
+        finite_ptrace_from s tl ->  
+        forall (s' : state) (iom oom : option message) (l : label),
+          verbose_valid_protocol_transition l s' s iom oom ->
+          finite_ptrace_from  s' ({| l := l; input := iom; destination := s; output := oom |} :: tl).
 
-      Lemma finite_ptrace_first_valid_transition
-            (s : state)
-            (tr : list in_state_out)
-            (te : in_state_out)
-            (Htr : finite_ptrace_from s (te :: tr))
-        : verbose_valid_protocol_transition (l te) s (destination te) (input te) (output te).
-      Proof.
-        inversion Htr. assumption.
-      Qed.
+    Lemma finite_ptrace_first_valid_transition
+          (s : state)
+          (tr : list in_state_out)
+          (te : in_state_out)
+          (Htr : finite_ptrace_from s (te :: tr))
+      : verbose_valid_protocol_transition (l te) s (destination te) (input te) (output te).
+    Proof.
+      inversion Htr. assumption.
+    Qed.
 
-      Lemma finite_ptrace_first_pstate
-        (s : state)
-        (tr : list in_state_out)
-        (Htr : finite_ptrace_from s tr)
-        : protocol_state_prop s
-        .
-      Proof.
-        inversion Htr; subst; try assumption.
-        - inversion H0. assumption.
-      Qed.
+    Lemma finite_ptrace_first_pstate
+      (s : state)
+      (tr : list in_state_out)
+      (Htr : finite_ptrace_from s tr)
+      : protocol_state_prop s
+      .
+    Proof.
+      inversion Htr; subst; try assumption.
+      - inversion H0. assumption.
+    Qed.
 
-      Lemma finite_ptrace_tail
-            (s : state)
-            (tr : list in_state_out)
-            (te : in_state_out)
-            (Htr : finite_ptrace_from s (te :: tr))
-        : finite_ptrace_from (destination te) tr.
-      Proof.
-        inversion Htr. assumption.
-      Qed.
+    Lemma finite_ptrace_tail
+          (s : state)
+          (tr : list in_state_out)
+          (te : in_state_out)
+          (Htr : finite_ptrace_from s (te :: tr))
+      : finite_ptrace_from (destination te) tr.
+    Proof.
+      inversion Htr. assumption.
+    Qed.
 
-      Lemma finite_ptrace_consecutive_valid_transition
-            (s : state)
-            (tr tr2 : list in_state_out)
-            (tr1 : list in_state_out)
-            (te1 te2 : in_state_out)
-            (Htr : finite_ptrace_from s tr)
-            (Heq : tr = tr1 ++ [te1; te2] ++ tr2)
-        : verbose_valid_protocol_transition (l te2) (destination te1) (destination te2) (input te2) (output te2).
-      Proof.
-        generalize dependent s. generalize dependent tr.
-        induction tr1.
-        - intros tr Heq s Htr. simpl in Heq; subst. inversion Htr; subst. inversion H2; subst. assumption.
-        - specialize (IHtr1 (tr1 ++ [te1; te2] ++ tr2) eq_refl).
-          intros tr Heq is Htr; subst. inversion Htr; subst.
-          simpl in IHtr1. specialize (IHtr1 s H2). assumption.
-      Qed.
+    Lemma finite_ptrace_consecutive_valid_transition
+          (s : state)
+          (tr tr2 : list in_state_out)
+          (tr1 : list in_state_out)
+          (te1 te2 : in_state_out)
+          (Htr : finite_ptrace_from s tr)
+          (Heq : tr = tr1 ++ [te1; te2] ++ tr2)
+      : verbose_valid_protocol_transition (l te2) (destination te1) (destination te2) (input te2) (output te2).
+    Proof.
+      generalize dependent s. generalize dependent tr.
+      induction tr1.
+      - intros tr Heq s Htr. simpl in Heq; subst. inversion Htr; subst. inversion H2; subst. assumption.
+      - specialize (IHtr1 (tr1 ++ [te1; te2] ++ tr2) eq_refl).
+        intros tr Heq is Htr; subst. inversion Htr; subst.
+        simpl in IHtr1. specialize (IHtr1 s H2). assumption.
+    Qed.
 
-      Definition finite_ptrace (s : state) (ls : list in_state_out) : Prop :=
-        finite_ptrace_from s ls /\ initial_state_prop s.
+    Definition finite_ptrace (s : state) (ls : list in_state_out) : Prop :=
+      finite_ptrace_from s ls /\ initial_state_prop s.
 
-      Lemma extend_right_finite_trace_from
-        : forall s1 ts s3 iom3 oom3 l3 (s2 := List.last (List.map destination ts) s1),
-          finite_ptrace_from s1 ts ->
-          verbose_valid_protocol_transition l3 s2 s3 iom3 oom3 ->
-          finite_ptrace_from s1 (ts ++ [{| l := l3; destination := s3; input := iom3; output := oom3 |}]).
-      Proof.
-        intros s1 ts s3 iom3 oom3 l3 s2 Ht12 Hv23.
-        induction Ht12.
-        - simpl. apply finite_ptrace_extend; try assumption.
-          constructor. apply (protocol_transition_destination Hv23).
-        - rewrite <- app_comm_cons.
-          apply finite_ptrace_extend; try assumption.
-          simpl in IHHt12. apply IHHt12.
-          unfold s2 in *; clear s2.
-          replace
-            (last (List.map destination tl) s)
-            with
-              (last (List.map destination ({| l := l1; input := iom; destination := s; output := oom |} :: tl)) s')
-          ; try assumption.
-          rewrite map_cons.
-          destruct tl; try reflexivity.
-          rewrite map_cons.
-          eapply remove_hd_last.
-      Qed.
+    Lemma extend_right_finite_trace_from
+      : forall s1 ts s3 iom3 oom3 l3 (s2 := List.last (List.map destination ts) s1),
+        finite_ptrace_from s1 ts ->
+        verbose_valid_protocol_transition l3 s2 s3 iom3 oom3 ->
+        finite_ptrace_from s1 (ts ++ [{| l := l3; destination := s3; input := iom3; output := oom3 |}]).
+    Proof.
+      intros s1 ts s3 iom3 oom3 l3 s2 Ht12 Hv23.
+      induction Ht12.
+      - simpl. apply finite_ptrace_extend; try assumption.
+        constructor. apply (protocol_transition_destination Hv23).
+      - rewrite <- app_comm_cons.
+        apply finite_ptrace_extend; try assumption.
+        simpl in IHHt12. apply IHHt12.
+        unfold s2 in *; clear s2.
+        replace
+          (last (List.map destination tl) s)
+          with
+            (last (List.map destination ({| l := l1; input := iom; destination := s; output := oom |} :: tl)) s')
+        ; try assumption.
+        rewrite map_cons.
+        destruct tl; try reflexivity.
+        rewrite map_cons.
+        eapply remove_hd_last.
+    Qed.
 
-      Lemma finite_ptrace_from_app_iff (s : state) (ls ls' : list in_state_out) (s' := (last (List.map destination ls) s))
-        : finite_ptrace_from s ls /\ finite_ptrace_from s' ls'
-          <->
-          finite_ptrace_from s (ls ++ ls').
-      Proof.
-        intros. generalize dependent ls'. generalize dependent s. 
-        induction ls; intros; split.
-        - intros [_ H]. assumption.
-        - simpl; intros; split; try assumption. constructor. inversion H; try assumption.
-          apply (protocol_transition_origin H1).
-        - simpl. intros [Htr Htr']. 
-          destruct a. apply finite_ptrace_extend.
-          + apply IHls. inversion Htr. split. apply H2.
-            unfold s' in Htr'. 
-            assert (last_identity: last (List.map destination ls) destination0 = last
-            (List.map destination
-               ({| l := l1; input := input0; destination := destination0; output := output0 |} :: ls)) s). {
-            rewrite map_cons. rewrite unroll_last. simpl. reflexivity. }
-            rewrite last_identity. assumption. 
-          + inversion Htr. apply H6.
-         - intros. inversion H. subst. specialize (IHls s1). simpl in IHls. specialize (IHls ls'). apply IHls in H3.
-           destruct H3. split. 
-           + constructor. apply H0. apply H4.
-           + assert (last_identity : s' = last (List.map destination ls) s1). {
-             unfold s'. rewrite map_cons. rewrite unroll_last. reflexivity. 
-           }
-           rewrite last_identity. assumption.
-      Qed.
+    Lemma finite_ptrace_from_app_iff (s : state) (ls ls' : list in_state_out) (s' := (last (List.map destination ls) s))
+      : finite_ptrace_from s ls /\ finite_ptrace_from s' ls'
+        <->
+        finite_ptrace_from s (ls ++ ls').
+    Proof.
+      intros. generalize dependent ls'. generalize dependent s. 
+      induction ls; intros; split.
+      - intros [_ H]. assumption.
+      - simpl; intros; split; try assumption. constructor. inversion H; try assumption.
+        apply (protocol_transition_origin H1).
+      - simpl. intros [Htr Htr']. 
+        destruct a. apply finite_ptrace_extend.
+        + apply IHls. inversion Htr. split. apply H2.
+          unfold s' in Htr'. 
+          assert (last_identity: last (List.map destination ls) destination0 = last
+          (List.map destination
+             ({| l := l1; input := input0; destination := destination0; output := output0 |} :: ls)) s). {
+          rewrite map_cons. rewrite unroll_last. simpl. reflexivity. }
+          rewrite last_identity. assumption. 
+        + inversion Htr. apply H6.
+       - intros. inversion H. subst. specialize (IHls s1). simpl in IHls. specialize (IHls ls'). apply IHls in H3.
+         destruct H3. split. 
+         + constructor. apply H0. apply H4.
+         + assert (last_identity : s' = last (List.map destination ls) s1). {
+           unfold s'. rewrite map_cons. rewrite unroll_last. reflexivity. 
+         }
+         rewrite last_identity. assumption.
+    Qed.
 
-      Lemma finite_ptrace_from_prefix
-        (s : state)
-        (ls : list in_state_out)       
-        (Htr : finite_ptrace_from s ls)
-        (n : nat)
-        : finite_ptrace_from s (list_prefix ls n).
-      Proof.
-        specialize (list_prefix_suffix ls n); intro Hdecompose.
-        rewrite <- Hdecompose in Htr.
-        apply finite_ptrace_from_app_iff in Htr.
-        destruct Htr as [Hpr _].
-        assumption.
-      Qed.
+    Lemma finite_ptrace_from_prefix
+      (s : state)
+      (ls : list in_state_out)       
+      (Htr : finite_ptrace_from s ls)
+      (n : nat)
+      : finite_ptrace_from s (list_prefix ls n).
+    Proof.
+      specialize (list_prefix_suffix ls n); intro Hdecompose.
+      rewrite <- Hdecompose in Htr.
+      apply finite_ptrace_from_app_iff in Htr.
+      destruct Htr as [Hpr _].
+      assumption.
+    Qed.
 
-      Lemma finite_ptrace_from_suffix
-        (s : state)
-        (ls : list in_state_out)       
-        (Htr : finite_ptrace_from s ls)
-        (n : nat)
-        (nth : state)
-        (Hnth : nth_error (s :: List.map destination ls) n = Some nth)
-        : finite_ptrace_from nth (list_suffix ls n)
-        .
-      Proof.
-        specialize (list_prefix_suffix ls n); intro Hdecompose.
-        rewrite <- Hdecompose in Htr.
-        apply finite_ptrace_from_app_iff in Htr.
-        destruct Htr as [_ Htr].
-        assert (Heq : last (List.map destination (list_prefix ls n)) s = nth).
-        { rewrite list_prefix_map.
-          destruct n.
-          - simpl in Hnth. inversion Hnth; subst; clear Hnth.
-            remember (List.map destination ls) as l.
-            destruct l; reflexivity.
-          - symmetry. apply list_prefix_nth_last.
-            simpl in Hnth. assumption.
-        }
-        rewrite Heq in Htr.
-        assumption.
-      Qed.
+    Lemma finite_ptrace_from_suffix
+      (s : state)
+      (ls : list in_state_out)       
+      (Htr : finite_ptrace_from s ls)
+      (n : nat)
+      (nth : state)
+      (Hnth : nth_error (s :: List.map destination ls) n = Some nth)
+      : finite_ptrace_from nth (list_suffix ls n)
+      .
+    Proof.
+      specialize (list_prefix_suffix ls n); intro Hdecompose.
+      rewrite <- Hdecompose in Htr.
+      apply finite_ptrace_from_app_iff in Htr.
+      destruct Htr as [_ Htr].
+      assert (Heq : last (List.map destination (list_prefix ls n)) s = nth).
+      { rewrite list_prefix_map.
+        destruct n.
+        - simpl in Hnth. inversion Hnth; subst; clear Hnth.
+          remember (List.map destination ls) as l.
+          destruct l; reflexivity.
+        - symmetry. apply list_prefix_nth_last.
+          simpl in Hnth. assumption.
+      }
+      rewrite Heq in Htr.
+      assumption.
+    Qed.
 
-      Lemma finite_ptrace_from_segment
-        (s : state)
-        (ls : list in_state_out)       
-        (Htr : finite_ptrace_from s ls)
-        (n1 n2 : nat)
-        (Hle : n1 <= n2)
-        (n1th : state)
-        (Hnth : nth_error (s :: List.map destination ls) n1 = Some n1th)
-        : finite_ptrace_from n1th (list_segment ls n1 n2).
-      Proof.
-        apply finite_ptrace_from_suffix with s.
-        - apply finite_ptrace_from_prefix. assumption.
-        - destruct n1; try assumption.
-          simpl. simpl in Hnth.
-          rewrite list_prefix_map.
-          rewrite list_prefix_nth; assumption.
-      Qed.
+    Lemma finite_ptrace_from_segment
+      (s : state)
+      (ls : list in_state_out)       
+      (Htr : finite_ptrace_from s ls)
+      (n1 n2 : nat)
+      (Hle : n1 <= n2)
+      (n1th : state)
+      (Hnth : nth_error (s :: List.map destination ls) n1 = Some n1th)
+      : finite_ptrace_from n1th (list_segment ls n1 n2).
+    Proof.
+      apply finite_ptrace_from_suffix with s.
+      - apply finite_ptrace_from_prefix. assumption.
+      - destruct n1; try assumption.
+        simpl. simpl in Hnth.
+        rewrite list_prefix_map.
+        rewrite list_prefix_nth; assumption.
+    Qed.
 
-      (* An infinite protocol trace originating in a given state *)
-      
-      CoInductive infinite_ptrace_from :
-        state -> Stream in_state_out -> Prop :=
-      | infinite_ptrace_extend : forall  (s : state) (tl : Stream in_state_out),
-          infinite_ptrace_from s tl ->  
-          forall (s' : state) (iom oom : option message) (l : label),
-            verbose_valid_protocol_transition l s' s iom oom ->
-            infinite_ptrace_from  s' (Cons {| l := l; input := iom; destination := s; output := oom |}  tl).
+    (* An infinite protocol trace originating in a given state *)
+    
+    CoInductive infinite_ptrace_from :
+      state -> Stream in_state_out -> Prop :=
+    | infinite_ptrace_extend : forall  (s : state) (tl : Stream in_state_out),
+        infinite_ptrace_from s tl ->  
+        forall (s' : state) (iom oom : option message) (l : label),
+          verbose_valid_protocol_transition l s' s iom oom ->
+          infinite_ptrace_from  s' (Cons {| l := l; input := iom; destination := s; output := oom |}  tl).
 
-      Lemma infinite_ptrace_consecutive_valid_transition 
-            (is : state)
-            (tr tr2 : Stream in_state_out)
-            (tr1 : list in_state_out)
-            (te1 te2 : in_state_out)
-            (Htr : infinite_ptrace_from is tr)
-            (Heq : tr = stream_app (tr1 ++ [te1; te2]) tr2)
-        : verbose_valid_protocol_transition (l te2) (destination te1) (destination te2) (input te2) (output te2).
-      Proof.
-        generalize dependent is. generalize dependent tr.
-        induction tr1.
-        - intros tr Heq is Htr. simpl in Heq; subst. inversion Htr; subst. inversion H2; subst. assumption.
-        - specialize (IHtr1 (stream_app (tr1 ++ [te1; te2]) tr2) eq_refl).
-          intros tr Heq is Htr; subst. inversion Htr; subst.
-          specialize (IHtr1 s H2). assumption.
-      Qed.
+    Lemma infinite_ptrace_consecutive_valid_transition 
+          (is : state)
+          (tr tr2 : Stream in_state_out)
+          (tr1 : list in_state_out)
+          (te1 te2 : in_state_out)
+          (Htr : infinite_ptrace_from is tr)
+          (Heq : tr = stream_app (tr1 ++ [te1; te2]) tr2)
+      : verbose_valid_protocol_transition (l te2) (destination te1) (destination te2) (input te2) (output te2).
+    Proof.
+      generalize dependent is. generalize dependent tr.
+      induction tr1.
+      - intros tr Heq is Htr. simpl in Heq; subst. inversion Htr; subst. inversion H2; subst. assumption.
+      - specialize (IHtr1 (stream_app (tr1 ++ [te1; te2]) tr2) eq_refl).
+        intros tr Heq is Htr; subst. inversion Htr; subst.
+        specialize (IHtr1 s H2). assumption.
+    Qed.
 
-      Lemma infinite_ptrace_from_app_iff
-        (s : state)
-        (ls : list in_state_out)
-        (ls' : Stream in_state_out)
-        (s' := (last (List.map destination ls) s))
-        : finite_ptrace_from s ls /\ infinite_ptrace_from s' ls'
-          <->
-          infinite_ptrace_from s (stream_app ls ls').
-      Proof.
-        intros. generalize dependent ls'. generalize dependent s. 
-        induction ls; intros; split.
-        - intros [_ H]. assumption.
-        - simpl; intros; split; try assumption. constructor. inversion H; try assumption.
-          apply (protocol_transition_origin H1).
-        - simpl. intros [Htr Htr']. 
-          destruct a. apply infinite_ptrace_extend.
-          + apply IHls. inversion Htr. split. apply H2.
-            unfold s' in Htr'. 
-            assert (last_identity: last (List.map destination ls) destination0 = last
-            (List.map destination
-               ({| l := l1; input := input0; destination := destination0; output := output0 |} :: ls)) s). {
-            rewrite map_cons. rewrite unroll_last. simpl. reflexivity. }
-            rewrite last_identity. assumption. 
-          + inversion Htr. apply H6.
-         - intros. inversion H. subst. specialize (IHls s1). simpl in IHls. specialize (IHls ls'). apply IHls in H3.
-           destruct H3. split. 
-           + constructor. apply H0. apply H4.
-           + assert (last_identity : s' = last (List.map destination ls) s1). {
-             unfold s'. rewrite map_cons. rewrite unroll_last. reflexivity. 
-           }
-           rewrite last_identity. assumption.
-      Qed.
+    Lemma infinite_ptrace_from_app_iff
+      (s : state)
+      (ls : list in_state_out)
+      (ls' : Stream in_state_out)
+      (s' := (last (List.map destination ls) s))
+      : finite_ptrace_from s ls /\ infinite_ptrace_from s' ls'
+        <->
+        infinite_ptrace_from s (stream_app ls ls').
+    Proof.
+      intros. generalize dependent ls'. generalize dependent s. 
+      induction ls; intros; split.
+      - intros [_ H]. assumption.
+      - simpl; intros; split; try assumption. constructor. inversion H; try assumption.
+        apply (protocol_transition_origin H1).
+      - simpl. intros [Htr Htr']. 
+        destruct a. apply infinite_ptrace_extend.
+        + apply IHls. inversion Htr. split. apply H2.
+          unfold s' in Htr'. 
+          assert (last_identity: last (List.map destination ls) destination0 = last
+          (List.map destination
+             ({| l := l1; input := input0; destination := destination0; output := output0 |} :: ls)) s). {
+          rewrite map_cons. rewrite unroll_last. simpl. reflexivity. }
+          rewrite last_identity. assumption. 
+        + inversion Htr. apply H6.
+       - intros. inversion H. subst. specialize (IHls s1). simpl in IHls. specialize (IHls ls'). apply IHls in H3.
+         destruct H3. split. 
+         + constructor. apply H0. apply H4.
+         + assert (last_identity : s' = last (List.map destination ls) s1). {
+           unfold s'. rewrite map_cons. rewrite unroll_last. reflexivity. 
+         }
+         rewrite last_identity. assumption.
+    Qed.
 
-      Lemma infinite_ptrace_from_prefix
-        (s : state)
-        (ls : Stream in_state_out)       
-        (Htr : infinite_ptrace_from s ls)
-        (n : nat)
-        : finite_ptrace_from s (stream_prefix ls n).
-      Proof.
-        specialize (stream_prefix_suffix ls n); intro Hdecompose.
-        rewrite <- Hdecompose in Htr.
-        apply infinite_ptrace_from_app_iff in Htr.
-        destruct Htr as [Hpr _].
-        assumption.
-      Qed.
+    Lemma infinite_ptrace_from_prefix
+      (s : state)
+      (ls : Stream in_state_out)       
+      (Htr : infinite_ptrace_from s ls)
+      (n : nat)
+      : finite_ptrace_from s (stream_prefix ls n).
+    Proof.
+      specialize (stream_prefix_suffix ls n); intro Hdecompose.
+      rewrite <- Hdecompose in Htr.
+      apply infinite_ptrace_from_app_iff in Htr.
+      destruct Htr as [Hpr _].
+      assumption.
+    Qed.
 
-      Lemma infinite_ptrace_from_segment
-        (s : state)
-        (ls : Stream in_state_out)       
-        (Htr : infinite_ptrace_from s ls)
-        (n1 n2 : nat)
-        (Hle : n1 <= n2)
-        (n1th := Str_nth n1 (Cons s (Streams.map destination ls)))
-        : finite_ptrace_from n1th (stream_segment ls n1 n2).
-      Proof.
-        apply finite_ptrace_from_suffix with s.
-        - apply infinite_ptrace_from_prefix. assumption.
-        - destruct n1; try reflexivity.
-          unfold n1th. clear n1th.
-          simpl.
-          rewrite stream_prefix_map.
-          rewrite stream_prefix_nth; try assumption.
-          reflexivity.
-      Qed.
+    Lemma infinite_ptrace_from_segment
+      (s : state)
+      (ls : Stream in_state_out)       
+      (Htr : infinite_ptrace_from s ls)
+      (n1 n2 : nat)
+      (Hle : n1 <= n2)
+      (n1th := Str_nth n1 (Cons s (Streams.map destination ls)))
+      : finite_ptrace_from n1th (stream_segment ls n1 n2).
+    Proof.
+      apply finite_ptrace_from_suffix with s.
+      - apply infinite_ptrace_from_prefix. assumption.
+      - destruct n1; try reflexivity.
+        unfold n1th. clear n1th.
+        simpl.
+        rewrite stream_prefix_map.
+        rewrite stream_prefix_nth; try assumption.
+        reflexivity.
+    Qed.
 
-      Definition infinite_ptrace (s : state) (st : Stream in_state_out)
-        := infinite_ptrace_from s st /\ initial_state_prop s.
+    Definition infinite_ptrace (s : state) (st : Stream in_state_out)
+      := infinite_ptrace_from s st /\ initial_state_prop s.
 
-      Inductive Trace : Type :=
-      | Finite : state -> list in_state_out -> Trace
-      | Infinite : state -> Stream in_state_out -> Trace.
+    Inductive Trace : Type :=
+    | Finite : state -> list in_state_out -> Trace
+    | Infinite : state -> Stream in_state_out -> Trace.
 
-      Definition trace_initial_state (tr : Trace) : state :=
-        match tr with 
-        | Finite s _ => s
-        | Infinite s _ => s
+    Definition trace_initial_state (tr : Trace) : state :=
+      match tr with 
+      | Finite s _ => s
+      | Infinite s _ => s
+      end. 
+
+    Definition protocol_trace_prop (tr : Trace) : Prop :=
+      match tr with 
+      | Finite s ls => finite_ptrace s ls
+      | Infinite s sm => infinite_ptrace s sm
+      end.
+
+    Definition ptrace_from_prop (tr : Trace) : Prop :=
+      match tr with 
+      | Finite s ls => finite_ptrace_from s ls
+      | Infinite s sm => infinite_ptrace_from s sm
+      end.
+
+    Definition protocol_trace : Type :=
+      { tr : Trace | protocol_trace_prop tr}.
+    
+    (* Protocol runs *) 
+    Record proto_run : Type := mk_proto_run
+                                 { start : initial_state
+                                   ; transitions : list in_state_out
+                                   ; final : state * option message
+                                 }.
+
+    Inductive vlsm_run_prop : proto_run -> Prop :=
+    | empty_run_initial_state
+        (is : initial_state)
+        (s : state := proj1_sig is)
+      : vlsm_run_prop {| start := is; transitions := []; final := (s, None) |}
+    | empty_run_initial_message
+        (im : initial_message)
+        (s : state := proj1_sig s0)
+        (om : option message := Some (proj1_sig im))
+      : vlsm_run_prop {| start := s0; transitions := []; final := (s, om) |}
+    | extend_run
+        (state_run : proto_run)
+        (Hs : vlsm_run_prop state_run)
+        (s := fst (final state_run))
+        (is := start state_run)
+        (ts := transitions state_run)
+        (msg_run : proto_run)
+        (Hm : vlsm_run_prop msg_run)
+        (om := snd (final msg_run))
+        (l : label)
+        (Hv : valid l (s, om))
+        (som' := transition l (s, om))
+      : vlsm_run_prop {| start := is; transitions := ts ++ [
+          {|   l := l
+          ;   input := om
+          ;   destination := fst som'
+          ;   output := snd som'
+          |}]; final := som' |}.
+
+    Definition vlsm_run : Type :=
+      { r : proto_run | vlsm_run_prop r }.
+
+
+    Lemma vlsm_run_last_state
+      (vr : vlsm_run)
+      (r := proj1_sig vr)
+      : last (List.map destination (transitions r)) (proj1_sig (start r)) = fst (final r).
+    Proof.
+      unfold r; clear r; destruct vr as [r Hr]; simpl.
+      induction Hr; simpl; try reflexivity.
+      rewrite map_app; simpl.
+      apply last_is_last.
+    Qed.
+
+    Lemma vlsm_run_last_final
+      (vr : vlsm_run)
+      (r := proj1_sig vr)
+      (tr := transitions r)
+      (Hne_tr : tr <> [])
+      (lst := last_error tr)
+      : option_map destination lst = Some (fst (final r))
+      /\ option_map output lst = Some (snd (final r)).
+    Proof.
+      unfold r in *; clear r; destruct vr as [r Hr]; inversion Hr; subst; simpl in *; clear Hr
+      ; try contradiction.
+      unfold tr in *. unfold lst in *. rewrite last_error_is_last . simpl.
+      split; reflexivity.
+    Qed.
+
+    Lemma run_is_protocol
+          (vr : vlsm_run)
+      : protocol_prop (final (proj1_sig vr)).
+    Proof.
+      destruct vr as [r Hr]; simpl.
+      induction Hr; simpl in *; try constructor.
+      unfold om in *; clear om. unfold s in *; clear s.
+      destruct (final state_run) as [s _om].
+      destruct (final msg_run) as [_s om].
+      specialize (protocol_generated l1 s _om IHHr1 _s om IHHr2 Hv). intro. assumption.
+    Qed.
+
+    Lemma protocol_is_run 
+          (som' : state * option message)
+          (Hp : protocol_prop som')
+      : exists vr : vlsm_run, (som' = final (proj1_sig vr)).
+    Proof.
+      induction Hp.
+      - exists (exist _ _ (empty_run_initial_state is)); reflexivity.
+      - exists (exist _ _ (empty_run_initial_message im)); reflexivity.
+      - destruct IHHp1 as [[state_run Hsr] Heqs]. destruct IHHp2 as [[msg_run Hmr] Heqm]. 
+        specialize (extend_run state_run Hsr). simpl. intros Hvr.
+        specialize (Hvr msg_run Hmr l1). simpl in Heqs. simpl in Heqm.
+        rewrite <- Heqs in Hvr. rewrite <- Heqm in Hvr. specialize (Hvr Hv).
+        exists (exist _ _ Hvr). reflexivity.
+    Qed.
+
+    Lemma run_is_trace
+          (vr : vlsm_run)
+          (r := proj1_sig vr)
+      : protocol_trace_prop (Finite (proj1_sig (start r)) (transitions r)).
+    Proof.
+      unfold r; clear r; destruct vr as [r Hr]; simpl.
+      induction Hr; simpl.
+      - specialize (protocol_initial_state is); intro Hpis; simpl in Hpis.
+        destruct is as [is His]; simpl. constructor; try assumption. constructor.
+        exists None. assumption.
+      - specialize (protocol_initial_state s0); intro Hps0; simpl in Hps0.
+        destruct s0 as [s0 Hs0]; simpl. constructor; try assumption. constructor.
+        exists None. assumption.
+      - destruct IHHr1 as [Htr Hinit].
+        split; try assumption.
+        apply extend_right_finite_trace_from; try assumption.
+        specialize vlsm_run_last_state; intros Hls. specialize (Hls (exist _ state_run Hr1)).
+        simpl in Hls. unfold ts. unfold is. rewrite Hls.
+        repeat split; try assumption.
+        + exists (snd (final state_run)). rewrite <- surjective_pairing.
+          specialize (run_is_protocol (exist _ state_run Hr1)); intro Hp; assumption.
+        + exists (fst (final msg_run)). rewrite <- surjective_pairing.
+          specialize (run_is_protocol (exist _ msg_run Hr2)); simpl; intro Hp; assumption.
+        + rewrite <- surjective_pairing. reflexivity.
+    Qed.
+
+    Lemma trace_is_run
+      (is : initial_state)
+      (tr : list in_state_out)
+      (Htr : finite_ptrace_from (proj1_sig is) tr)
+      : exists r : proto_run,
+        vlsm_run_prop r /\
+        start r = is /\ transitions r = tr
+      .
+    Proof.
+      generalize dependent tr.
+      apply (rev_ind (fun tr => (finite_ptrace_from (proj1_sig is) tr ->
+                exists r : proto_run, vlsm_run_prop r /\ start r = is /\ transitions r = tr))).
+      - intros H.
+        exists {| start := is; transitions := []; final := (proj1_sig is, None) |}; simpl; repeat split; try reflexivity.
+        apply empty_run_initial_state.
+      - intros lst prefix IHprefix H. 
+        apply finite_ptrace_from_app_iff in H.
+        destruct H as [Hprefix Hlst].
+        specialize (IHprefix Hprefix).
+        destruct IHprefix as [r0 [Hr0 [Hstart Htr_r0]]].
+        exists {| start := is; transitions := prefix ++ [lst]; final := (destination lst, output lst) |}.
+        simpl. repeat split; try reflexivity.
+        specialize (extend_run r0 Hr0); simpl; intro Hextend.
+        apply finite_ptrace_first_valid_transition in Hlst.
+        destruct lst as [lst_l lst_in lst_dest lst_out].
+        simpl in *.
+        specialize (vlsm_run_last_state (exist _ r0 Hr0)); intro Hlast_state.
+        simpl in Hlast_state. rewrite Htr_r0 in Hlast_state.
+        rewrite Hstart in Hlast_state. rewrite Hlast_state in Hlst.
+        specialize (protocol_prop_transition_in Hlst); intro Hmsg.
+        destruct Hmsg as [_s Hmsg].
+        apply protocol_is_run in Hmsg.
+        destruct Hmsg as [[r_msg Hr_msg] Hmsg].
+        specialize (Hextend r_msg Hr_msg lst_l).
+        specialize (protocol_transition_valid Hlst); intro Hvalid.
+        simpl in Hmsg. rewrite <- Hmsg in Hextend. simpl  in Hextend.
+        specialize (Hextend Hvalid). rewrite Hstart in Hextend.
+        specialize (protocol_transition_transition Hlst); intro Htransition.
+        rewrite Htransition in Hextend. simpl in Hextend.
+        rewrite Htr_r0 in Hextend.
+        apply Hextend.
+        Qed.
+
+    (* protocol states/messages correspond to protocol traces *)
+
+    Lemma protocol_is_trace
+          (som' : state * option message)
+          (Hp : protocol_prop som')
+          (s' := fst som')
+          (om' := snd som')
+         
+      : initial_state_prop s' \/ exists (is : state) (tr : list in_state_out),
+            finite_ptrace is tr
+            /\ option_map destination (last_error tr) = Some s'
+            /\ option_map output (last_error tr) = Some om'.
+    Proof.
+      specialize (protocol_is_run som' Hp); intros [vr Heq].
+      specialize (run_is_trace vr); simpl; intros Htr.
+      destruct vr as [r Hvr]; simpl in *.
+      destruct (transitions r) eqn:Htrace.
+      - inversion Hvr; subst; simpl in Htrace. 
+        + destruct is as [s0 His]. left. assumption.
+        + destruct s0 as [s0 His]. left. assumption.
+        + destruct ts; inversion Htrace.
+      - right. exists (proj1_sig (start r)). exists (transitions r). rewrite Htrace.
+        split; try assumption.
+        specialize (vlsm_run_last_final (exist _ r Hvr)); simpl; rewrite Htrace; simpl.
+        rewrite <- Heq.
+        intros Hlf; apply Hlf. intros HC; inversion HC.
+    Qed. 
+
+    (* Projections of traces *)
+    Inductive Trace_states : Type :=
+    | Finite_states : list state -> Trace_states
+    | Infinite_states : Stream state -> Trace_states.
+
+    Definition trace_nth (tr : Trace)
+      : nat -> option state :=
+      fun (n : nat) =>
+        match tr with
+        | Finite s ls => nth_error (s::List.map destination ls) n
+        | Infinite s st => Some (Str_nth n (Cons s (Streams.map destination st)))
         end. 
 
-      Definition ptrace_prop (tr : Trace) : Prop :=
-        match tr with 
-        | Finite s ls => finite_ptrace s ls
-        | Infinite s sm => infinite_ptrace s sm
-        end.
+    Definition protocol_state_trace (tr : protocol_trace) : Trace_states :=
+      match proj1_sig tr with
+      | Finite s ls => Finite_states (s :: List.map destination ls)
+      | Infinite s st => Infinite_states (Cons s (map destination st)) end.
+    
+    Definition protocol_state_trace_prop (tr : Trace_states)
+      := exists (ptr : protocol_trace), tr = protocol_state_trace ptr.
+    
 
-      Definition ptrace_from_prop (tr : Trace) : Prop :=
-        match tr with 
-        | Finite s ls => finite_ptrace_from s ls
-        | Infinite s sm => infinite_ptrace_from s sm
-        end.
+    Definition in_futures
+      (pfirst psecond : protocol_state)
+      (first := proj1_sig pfirst)
+      (second := proj1_sig psecond)
+      : Prop :=
+      exists (tr : list in_state_out),
+        finite_ptrace_from first tr /\
+        last (List.map destination tr) first = second.
 
-      Definition protocol_trace : Type :=
-        { tr : Trace | ptrace_prop tr}.
-      
-      (* Protocol runs *) 
-      Record proto_run : Type := mk_proto_run
-                                   { start : initial_state
-                                     ; transitions : list in_state_out
-                                     ; final : state * option message
-                                   }.
-
-      Inductive vlsm_run_prop : proto_run -> Prop :=
-      | empty_run_initial_state
-          (is : initial_state)
-          (s : state := proj1_sig is)
-        : vlsm_run_prop {| start := is; transitions := []; final := (s, None) |}
-      | empty_run_initial_message
-          (im : initial_message)
-          (s : state := proj1_sig s0)
-          (om : option message := Some (proj1_sig im))
-        : vlsm_run_prop {| start := s0; transitions := []; final := (s, om) |}
-      | extend_run
-          (state_run : proto_run)
-          (Hs : vlsm_run_prop state_run)
-          (s := fst (final state_run))
-          (is := start state_run)
-          (ts := transitions state_run)
-          (msg_run : proto_run)
-          (Hm : vlsm_run_prop msg_run)
-          (om := snd (final msg_run))
-          (l : label)
-          (Hv : valid l (s, om))
-          (som' := transition l (s, om))
-        : vlsm_run_prop {| start := is; transitions := ts ++ [
-            {|   l := l
-            ;   input := om
-            ;   destination := fst som'
-            ;   output := snd som'
-            |}]; final := som' |}.
-
-      Definition vlsm_run : Type :=
-        { r : proto_run | vlsm_run_prop r }.
-
-
-      Lemma vlsm_run_last_state
-        (vr : vlsm_run)
-        (r := proj1_sig vr)
-        : last (List.map destination (transitions r)) (proj1_sig (start r)) = fst (final r).
-      Proof.
-        unfold r; clear r; destruct vr as [r Hr]; simpl.
-        induction Hr; simpl; try reflexivity.
-        rewrite map_app; simpl.
-        apply last_is_last.
-      Qed.
-
-      Lemma vlsm_run_last_final
-        (vr : vlsm_run)
-        (r := proj1_sig vr)
-        (tr := transitions r)
-        (Hne_tr : tr <> [])
-        (lst := last_error tr)
-        : option_map destination lst = Some (fst (final r))
-        /\ option_map output lst = Some (snd (final r)).
-      Proof.
-        unfold r in *; clear r; destruct vr as [r Hr]; inversion Hr; subst; simpl in *; clear Hr
-        ; try contradiction.
-        unfold tr in *. unfold lst in *. rewrite last_error_is_last . simpl.
-        split; reflexivity.
-      Qed.
-
-      Lemma run_is_protocol
-            (vr : vlsm_run)
-        : protocol_prop (final (proj1_sig vr)).
-      Proof.
-        destruct vr as [r Hr]; simpl.
-        induction Hr; simpl in *; try constructor.
-        unfold om in *; clear om. unfold s in *; clear s.
-        destruct (final state_run) as [s _om].
-        destruct (final msg_run) as [_s om].
-        specialize (protocol_generated l1 s _om IHHr1 _s om IHHr2 Hv). intro. assumption.
-      Qed.
-
-      Lemma protocol_is_run 
-            (som' : state * option message)
-            (Hp : protocol_prop som')
-        : exists vr : vlsm_run, (som' = final (proj1_sig vr)).
-      Proof.
-        induction Hp.
-        - exists (exist _ _ (empty_run_initial_state is)); reflexivity.
-        - exists (exist _ _ (empty_run_initial_message im)); reflexivity.
-        - destruct IHHp1 as [[state_run Hsr] Heqs]. destruct IHHp2 as [[msg_run Hmr] Heqm]. 
-          specialize (extend_run state_run Hsr). simpl. intros Hvr.
-          specialize (Hvr msg_run Hmr l1). simpl in Heqs. simpl in Heqm.
-          rewrite <- Heqs in Hvr. rewrite <- Heqm in Hvr. specialize (Hvr Hv).
-          exists (exist _ _ Hvr). reflexivity.
-      Qed.
-
-      Lemma run_is_trace
-            (vr : vlsm_run)
-            (r := proj1_sig vr)
-        : ptrace_prop (Finite (proj1_sig (start r)) (transitions r)).
-      Proof.
-        unfold r; clear r; destruct vr as [r Hr]; simpl.
-        induction Hr; simpl.
-        - specialize (protocol_initial_state is); intro Hpis; simpl in Hpis.
-          destruct is as [is His]; simpl. constructor; try assumption. constructor.
-          exists None. assumption.
-        - specialize (protocol_initial_state s0); intro Hps0; simpl in Hps0.
-          destruct s0 as [s0 Hs0]; simpl. constructor; try assumption. constructor.
-          exists None. assumption.
-        - destruct IHHr1 as [Htr Hinit].
-          split; try assumption.
-          apply extend_right_finite_trace_from; try assumption.
-          specialize vlsm_run_last_state; intros Hls. specialize (Hls (exist _ state_run Hr1)).
-          simpl in Hls. unfold ts. unfold is. rewrite Hls.
-          repeat split; try assumption.
-          + exists (snd (final state_run)). rewrite <- surjective_pairing.
-            specialize (run_is_protocol (exist _ state_run Hr1)); intro Hp; assumption.
-          + exists (fst (final msg_run)). rewrite <- surjective_pairing.
-            specialize (run_is_protocol (exist _ msg_run Hr2)); simpl; intro Hp; assumption.
-          + rewrite <- surjective_pairing. reflexivity.
-      Qed.
-
-      Lemma trace_is_run
-        (is : initial_state)
-        (tr : list in_state_out)
-        (Htr : finite_ptrace_from (proj1_sig is) tr)
-        : exists r : proto_run,
-          vlsm_run_prop r /\
-          start r = is /\ transitions r = tr
-        .
-      Proof.
-        generalize dependent tr.
-        apply (rev_ind (fun tr => (finite_ptrace_from (proj1_sig is) tr ->
-                  exists r : proto_run, vlsm_run_prop r /\ start r = is /\ transitions r = tr))).
-        - intros H.
-          exists {| start := is; transitions := []; final := (proj1_sig is, None) |}; simpl; repeat split; try reflexivity.
-          apply empty_run_initial_state.
-        - intros lst prefix IHprefix H. 
-          apply finite_ptrace_from_app_iff in H.
-          destruct H as [Hprefix Hlst].
-          specialize (IHprefix Hprefix).
-          destruct IHprefix as [r0 [Hr0 [Hstart Htr_r0]]].
-          exists {| start := is; transitions := prefix ++ [lst]; final := (destination lst, output lst) |}.
-          simpl. repeat split; try reflexivity.
-          specialize (extend_run r0 Hr0); simpl; intro Hextend.
-          apply finite_ptrace_first_valid_transition in Hlst.
-          destruct lst as [lst_l lst_in lst_dest lst_out].
-          simpl in *.
-          specialize (vlsm_run_last_state (exist _ r0 Hr0)); intro Hlast_state.
-          simpl in Hlast_state. rewrite Htr_r0 in Hlast_state.
-          rewrite Hstart in Hlast_state. rewrite Hlast_state in Hlst.
-          specialize (protocol_prop_transition_in Hlst); intro Hmsg.
-          destruct Hmsg as [_s Hmsg].
-          apply protocol_is_run in Hmsg.
-          destruct Hmsg as [[r_msg Hr_msg] Hmsg].
-          specialize (Hextend r_msg Hr_msg lst_l).
-          specialize (protocol_transition_valid Hlst); intro Hvalid.
-          simpl in Hmsg. rewrite <- Hmsg in Hextend. simpl  in Hextend.
-          specialize (Hextend Hvalid). rewrite Hstart in Hextend.
-          specialize (protocol_transition_transition Hlst); intro Htransition.
-          rewrite Htransition in Hextend. simpl in Hextend.
-          rewrite Htr_r0 in Hextend.
-          apply Hextend.
-          Qed.
-
-      (* protocol states/messages correspond to protocol traces *)
-
-      Lemma protocol_is_trace
-            (som' : state * option message)
-            (Hp : protocol_prop som')
-            (s' := fst som')
-            (om' := snd som')
-           
-        : initial_state_prop s' \/ exists (is : state) (tr : list in_state_out),
-              finite_ptrace is tr
-              /\ option_map destination (last_error tr) = Some s'
-              /\ option_map output (last_error tr) = Some om'.
-      Proof.
-        specialize (protocol_is_run som' Hp); intros [vr Heq].
-        specialize (run_is_trace vr); simpl; intros Htr.
-        destruct vr as [r Hvr]; simpl in *.
-        destruct (transitions r) eqn:Htrace.
-        - inversion Hvr; subst; simpl in Htrace. 
-          + destruct is as [s0 His]. left. assumption.
-          + destruct s0 as [s0 His]. left. assumption.
-          + destruct ts; inversion Htrace.
-        - right. exists (proj1_sig (start r)). exists (transitions r). rewrite Htrace.
-          split; try assumption.
-          specialize (vlsm_run_last_final (exist _ r Hvr)); simpl; rewrite Htrace; simpl.
-          rewrite <- Heq.
-          intros Hlf; apply Hlf. intros HC; inversion HC.
-      Qed. 
-
-      (* Projections of traces *)
-      Inductive Trace_states : Type :=
-      | Finite_states : list state -> Trace_states
-      | Infinite_states : Stream state -> Trace_states.
-
-      Definition trace_nth (tr : Trace)
-        : nat -> option state :=
-        fun (n : nat) =>
-          match tr with
-          | Finite s ls => nth_error (s::List.map destination ls) n
-          | Infinite s st => Some (Str_nth n (Cons s (Streams.map destination st)))
-          end. 
-
-      Definition protocol_state_trace (tr : protocol_trace) : Trace_states :=
-        match proj1_sig tr with
-        | Finite s ls => Finite_states (s :: List.map destination ls)
-        | Infinite s st => Infinite_states (Cons s (map destination st)) end.
-      
-      Definition protocol_state_trace_prop (tr : Trace_states)
-        := exists (ptr : protocol_trace), tr = protocol_state_trace ptr.
-      
-
-      Definition in_futures
-        (pfirst psecond : protocol_state)
-        (first := proj1_sig pfirst)
-        (second := proj1_sig psecond)
-        : Prop :=
-        exists (tr : list in_state_out),
-          finite_ptrace_from first tr /\
-          last (List.map destination tr) first = second.
-
-      Lemma in_futures_witness
-        (pfirst psecond : protocol_state)
-        (first := proj1_sig pfirst)
-        (second := proj1_sig psecond)
-        (Hfutures : in_futures pfirst psecond)
-        : exists (tr : protocol_trace) (n1 n2 : nat),
-          n1 <= n2
-          /\ trace_nth (proj1_sig tr) n1 = Some first
-          /\ trace_nth (proj1_sig tr) n2 = Some second.
-      Proof.
-        unfold first in *; clear first. unfold second in *; clear second.
-        destruct pfirst as [first [_mfirst Hfirst]].
-        destruct psecond as [second [_msecond Hsecond]].
-        simpl.
-        unfold in_futures in Hfutures. simpl in Hfutures.
-        destruct Hfutures as [suffix_tr [Hsuffix_tr Hsnd]].
-        apply protocol_is_run in Hfirst.
-        destruct Hfirst as [prefix_run Hprefix_run].
-        specialize (vlsm_run_last_state prefix_run); intro Hprefix_last.
-        specialize (run_is_trace prefix_run); intro Hprefix_tr.
-        destruct prefix_run as [prefix_run Hpref_run].
-        destruct prefix_run as [prefix_start prefix_tr prefix_final].
+    Lemma in_futures_witness
+      (pfirst psecond : protocol_state)
+      (first := proj1_sig pfirst)
+      (second := proj1_sig psecond)
+      (Hfutures : in_futures pfirst psecond)
+      : exists (tr : protocol_trace) (n1 n2 : nat),
+        n1 <= n2
+        /\ trace_nth (proj1_sig tr) n1 = Some first
+        /\ trace_nth (proj1_sig tr) n2 = Some second.
+    Proof.
+      unfold first in *; clear first. unfold second in *; clear second.
+      destruct pfirst as [first [_mfirst Hfirst]].
+      destruct psecond as [second [_msecond Hsecond]].
+      simpl.
+      unfold in_futures in Hfutures. simpl in Hfutures.
+      destruct Hfutures as [suffix_tr [Hsuffix_tr Hsnd]].
+      apply protocol_is_run in Hfirst.
+      destruct Hfirst as [prefix_run Hprefix_run].
+      specialize (vlsm_run_last_state prefix_run); intro Hprefix_last.
+      specialize (run_is_trace prefix_run); intro Hprefix_tr.
+      destruct prefix_run as [prefix_run Hpref_run].
+      destruct prefix_run as [prefix_start prefix_tr prefix_final].
+      subst; simpl in *.
+      specialize (finite_ptrace_from_app_iff (proj1_sig prefix_start) prefix_tr suffix_tr); intro Happ.
+      simpl in Happ.
+      rewrite Hprefix_last in Happ. rewrite <- Hprefix_run in Happ.
+      simpl in Happ.
+      destruct Happ as [Happ _].
+      destruct Hprefix_tr as [Hprefix_tr Hinit].
+      specialize (Happ (conj Hprefix_tr Hsuffix_tr)).
+      assert (Hfinite_tr: finite_ptrace (proj1_sig prefix_start) (prefix_tr ++ suffix_tr))
+        by (constructor; assumption).
+      assert (Htr : protocol_trace_prop (Finite (proj1_sig prefix_start) (prefix_tr ++ suffix_tr)))
+        by assumption.
+      exists (exist _ (Finite (proj1_sig prefix_start) (prefix_tr ++ suffix_tr)) Htr).
+      simpl.
+      exists (length prefix_tr).
+      exists (length prefix_tr + length suffix_tr).
+      remember (length prefix_tr) as m.
+      split; try apply le_plus_l.
+      destruct m; simpl.
+      + symmetry in Heqm. apply length_zero_iff_nil in Heqm.
         subst; simpl in *.
-        specialize (finite_ptrace_from_app_iff (proj1_sig prefix_start) prefix_tr suffix_tr); intro Happ.
-        simpl in Happ.
-        rewrite Hprefix_last in Happ. rewrite <- Hprefix_run in Happ.
-        simpl in Happ.
-        destruct Happ as [Happ _].
-        destruct Hprefix_tr as [Hprefix_tr Hinit].
-        specialize (Happ (conj Hprefix_tr Hsuffix_tr)).
-        assert (Hfinite_tr: finite_ptrace (proj1_sig prefix_start) (prefix_tr ++ suffix_tr))
-          by (constructor; assumption).
-        assert (Htr : ptrace_prop (Finite (proj1_sig prefix_start) (prefix_tr ++ suffix_tr)))
-          by assumption.
-        exists (exist _ (Finite (proj1_sig prefix_start) (prefix_tr ++ suffix_tr)) Htr).
-        simpl.
-        exists (length prefix_tr).
-        exists (length prefix_tr + length suffix_tr).
-        remember (length prefix_tr) as m.
-        split; try apply le_plus_l.
-        destruct m; simpl.
-        + symmetry in Heqm. apply length_zero_iff_nil in Heqm.
-          subst; simpl in *.
-          split; try (f_equal; assumption).
-          remember (length suffix_tr) as delta.
-          destruct delta; simpl.
-          * symmetry in Heqdelta. apply length_zero_iff_nil in Heqdelta.
-            subst; simpl in *. f_equal.
-          * apply nth_error_last.
-            rewrite map_length. assumption.
-        + rewrite map_app. 
-          assert (Hnth_pref : forall suf, nth_error (List.map destination prefix_tr ++ suf) m = Some first).
-          { intro. rewrite nth_error_app1.
-            - specialize (nth_error_last (List.map destination prefix_tr) m); intro Hnth.
-              assert (Hlen : S m = length (List.map destination prefix_tr))
-                by (rewrite map_length; assumption).
-              specialize (Hnth Hlen (proj1_sig prefix_start)).
-              rewrite Hnth. f_equal. subst.
-              rewrite Hprefix_last. reflexivity.
-            - rewrite map_length. rewrite <- Heqm. constructor.
+        split; try (f_equal; assumption).
+        remember (length suffix_tr) as delta.
+        destruct delta; simpl.
+        * symmetry in Heqdelta. apply length_zero_iff_nil in Heqdelta.
+          subst; simpl in *. f_equal.
+        * apply nth_error_last.
+          rewrite map_length. assumption.
+      + rewrite map_app. 
+        assert (Hnth_pref : forall suf, nth_error (List.map destination prefix_tr ++ suf) m = Some first).
+        { intro. rewrite nth_error_app1.
+          - specialize (nth_error_last (List.map destination prefix_tr) m); intro Hnth.
+            assert (Hlen : S m = length (List.map destination prefix_tr))
+              by (rewrite map_length; assumption).
+            specialize (Hnth Hlen (proj1_sig prefix_start)).
+            rewrite Hnth. f_equal. subst.
+            rewrite Hprefix_last. reflexivity.
+          - rewrite map_length. rewrite <- Heqm. constructor.
+        }
+        split; try apply Hnth_pref.
+        remember (length suffix_tr) as delta.
+        destruct delta; simpl.
+        * symmetry in Heqdelta. apply length_zero_iff_nil in Heqdelta.
+          subst; simpl in *. rewrite plus_0_r.
+          apply Hnth_pref.
+        * { rewrite nth_error_app2.
+            - rewrite map_length.
+              rewrite <- Heqm. 
+              assert (Hdelta : m + S delta - S m = delta)
+                by (rewrite <- plus_Snm_nSm; apply minus_plus).
+              rewrite Hdelta.
+              specialize (nth_error_last (List.map destination suffix_tr) delta); intro Hnth.
+              rewrite map_length in Hnth.
+              specialize (Hnth Heqdelta first).
+              assumption.
+            - rewrite map_length. rewrite <- Heqm.
+              rewrite <- plus_Snm_nSm. simpl.
+              apply le_n_S. apply le_plus_l.
           }
-          split; try apply Hnth_pref.
-          remember (length suffix_tr) as delta.
-          destruct delta; simpl.
-          * symmetry in Heqdelta. apply length_zero_iff_nil in Heqdelta.
-            subst; simpl in *. rewrite plus_0_r.
-            apply Hnth_pref.
-          * { rewrite nth_error_app2.
-              - rewrite map_length.
-                rewrite <- Heqm. 
-                assert (Hdelta : m + S delta - S m = delta)
-                  by (rewrite <- plus_Snm_nSm; apply minus_plus).
-                rewrite Hdelta.
-                specialize (nth_error_last (List.map destination suffix_tr) delta); intro Hnth.
-                rewrite map_length in Hnth.
-                specialize (Hnth Heqdelta first).
-                assumption.
-              - rewrite map_length. rewrite <- Heqm.
-                rewrite <- plus_Snm_nSm. simpl.
-                apply le_n_S. apply le_plus_l.
-            }
-      Qed.
+    Qed.
 
-      Definition trace_segment
-        (tr : Trace)
-        (n1 n2 : nat)
-        : list in_state_out
-        := match tr with
-        | Finite s l => list_segment l n1 n2
-        | Infinite s l => stream_segment l n1 n2
+    Definition trace_segment
+      (tr : Trace)
+      (n1 n2 : nat)
+      : list in_state_out
+      := match tr with
+      | Finite s l => list_segment l n1 n2
+      | Infinite s l => stream_segment l n1 n2
+      end.
+
+    Lemma ptrace_segment
+      (tr : Trace)
+      (Htr : protocol_trace_prop tr)
+      (n1 n2 : nat)
+      (Hle : n1 <= n2)
+      (first : state)
+      (Hfirst : trace_nth tr n1 = Some first)
+      : finite_ptrace_from first (trace_segment tr n1 n2).
+    Proof.
+      destruct tr as [s tr | s tr]; simpl in *; destruct Htr as [Htr Hinit].
+      - apply finite_ptrace_from_segment with s; try assumption.
+      - inversion Hfirst; subst; clear Hfirst.
+        apply (infinite_ptrace_from_segment s tr Htr n1 n2 Hle).
+    Qed.
+
+    Lemma in_futures_witness_reverse
+      (pfirst psecond : protocol_state)
+      (first := proj1_sig pfirst)
+      (second := proj1_sig psecond)
+      (H : exists (tr : protocol_trace) (n1 n2 : nat),
+        n1 <= n2
+        /\ trace_nth (proj1_sig tr) n1 = Some first
+        /\ trace_nth (proj1_sig tr) n2 = Some second
+      )
+      : in_futures pfirst psecond.
+    Proof.
+      destruct H as [[tr Htr] [n1 [n2 [Hle [Hs1 Hs2]]]]].
+      unfold in_futures. unfold first in *. clear first.
+      unfold second in *. clear second.
+      destruct pfirst as [first Hfirst].
+      destruct psecond as [second Hsecond].
+      simpl in *.
+      inversion Hle; subst; clear Hle.
+      - rewrite Hs1 in Hs2. inversion Hs2; subst; clear Hs2.
+        exists []. split.
+        + constructor. assumption.
+        + reflexivity.
+      -  exists (trace_segment tr n1 (S m)).
+        split.
+        + apply ptrace_segment; try assumption. constructor. assumption.
+        + { destruct tr as [s tr | s tr]; simpl.
+          - unfold list_segment.
+            rewrite list_suffix_map. rewrite list_prefix_map.
+            simpl in Hs2.
+            rewrite list_suffix_last.
+            + symmetry. apply list_prefix_nth_last. assumption.
+            + apply nth_error_length in Hs2.
+              specialize (list_prefix_length (List.map destination tr) (S m) Hs2); intro Hpref_len.
+              rewrite Hpref_len. 
+              apply le_n_S. assumption.
+          - unfold stream_segment.
+            rewrite list_suffix_map. rewrite stream_prefix_map.
+            simpl in Hs2.
+            rewrite list_suffix_last.
+            + symmetry. rewrite stream_prefix_nth_last.
+              unfold Str_nth in Hs2. simpl in Hs2.
+              inversion Hs2; subst.
+              reflexivity.
+            + specialize (stream_prefix_length (Streams.map destination tr) (S m)); intro Hpref_len.
+              rewrite Hpref_len. 
+              apply le_n_S. assumption.
+          }
+    Qed.
+
+    Definition trace_last (tr : Trace) : option state
+      :=
+        match tr with
+        | Finite s ls => Some (last (List.map destination ls) s)
+        | Infinite _ _ => None
         end.
 
-      Lemma ptrace_segment
-        (tr : Trace)
-        (Htr : ptrace_prop tr)
-        (n1 n2 : nat)
-        (Hle : n1 <= n2)
-        (first : state)
-        (Hfirst : trace_nth tr n1 = Some first)
-        : finite_ptrace_from first (trace_segment tr n1 n2).
-      Proof.
-        destruct tr as [s tr | s tr]; simpl in *; destruct Htr as [Htr Hinit].
-        - apply finite_ptrace_from_segment with s; try assumption.
-        - inversion Hfirst; subst; clear Hfirst.
-          apply (infinite_ptrace_from_segment s tr Htr n1 n2 Hle).
-      Qed.
+    Definition trace_first (tr : Trace) : state
+      :=
+        match tr with
+        | Finite s _ => s
+        | Infinite s _ => s
+        end.
 
-      Lemma in_futures_witness_reverse
-        (pfirst psecond : protocol_state)
-        (first := proj1_sig pfirst)
-        (second := proj1_sig psecond)
-        (H : exists (tr : protocol_trace) (n1 n2 : nat),
-          n1 <= n2
-          /\ trace_nth (proj1_sig tr) n1 = Some first
-          /\ trace_nth (proj1_sig tr) n2 = Some second
-        )
-        : in_futures pfirst psecond.
-      Proof.
-        destruct H as [[tr Htr] [n1 [n2 [Hle [Hs1 Hs2]]]]].
-        unfold in_futures. unfold first in *. clear first.
-        unfold second in *. clear second.
-        destruct pfirst as [first Hfirst].
-        destruct psecond as [second Hsecond].
-        simpl in *.
-        inversion Hle; subst; clear Hle.
-        - rewrite Hs1 in Hs2. inversion Hs2; subst; clear Hs2.
-          exists []. split.
-          + constructor. assumption.
-          + reflexivity.
-        -  exists (trace_segment tr n1 (S m)).
-          split.
-          + apply ptrace_segment; try assumption. constructor. assumption.
-          + { destruct tr as [s tr | s tr]; simpl.
-            - unfold list_segment.
-              rewrite list_suffix_map. rewrite list_prefix_map.
-              simpl in Hs2.
-              rewrite list_suffix_last.
-              + symmetry. apply list_prefix_nth_last. assumption.
-              + apply nth_error_length in Hs2.
-                specialize (list_prefix_length (List.map destination tr) (S m) Hs2); intro Hpref_len.
-                rewrite Hpref_len. 
-                apply le_n_S. assumption.
-            - unfold stream_segment.
-              rewrite list_suffix_map. rewrite stream_prefix_map.
-              simpl in Hs2.
-              rewrite list_suffix_last.
-              + symmetry. rewrite stream_prefix_nth_last.
-                unfold Str_nth in Hs2. simpl in Hs2.
-                inversion Hs2; subst.
-                reflexivity.
-              + specialize (stream_prefix_length (Streams.map destination tr) (S m)); intro Hpref_len.
-                rewrite Hpref_len. 
-                apply le_n_S. assumption.
-            }
-      Qed.
+    Inductive Trace_messages : Type :=
+    | Finite_messages : list (option message) -> Trace_messages
+    | Infinite_messages : Stream (option message) -> Trace_messages. 
 
-      Definition trace_last (tr : Trace) : option state
-        :=
-          match tr with
-          | Finite s ls => Some (last (List.map destination ls) s)
-          | Infinite _ _ => None
+    Definition protocol_output_messages_trace (tr : protocol_trace) : Trace_messages :=
+      match proj1_sig tr with
+      | Finite _ ls => Finite_messages (List.map output ls)
+      | Infinite _ st => Infinite_messages (map output st) end.
+
+    Definition protocol_input_messages_trace (tr : protocol_trace) : Trace_messages :=
+      match proj1_sig tr with
+      | Finite _ ls => Finite_messages (List.map input ls)
+      | Infinite _ st => Infinite_messages (map input st) end.
+
+    (* Defining equivocation on these trace definitions *)
+    (* Section 7 :
+       A message m received by a protocol state s with a transition label l in a
+       protocol execution trace is called "an equivocation" if it wasn't produced
+       in that trace
+    *)
+
+    Definition trace_prefix
+               (tr : Trace)
+               (last : in_state_out)
+               (prefix : list in_state_out)
+      :=
+        match tr with
+        | Finite s ls => exists suffix, ls = prefix ++ (last :: suffix)
+        | Infinite s st => exists suffix, st = stream_app prefix (Cons last suffix)
+        end.
+
+    (** A finite trace is terminating if there's no other trace that contains it
+        as a (proper) prefix.
+    **)
+
+    Definition terminating_trace_prop (tr : Trace) : Prop 
+       :=
+         match tr with 
+         | Finite s ls => 
+             (exists (tr : protocol_trace) 
+             (last : in_state_out), 
+             trace_prefix (proj1_sig tr) last ls) -> False 
+         | Infinite s ls => False
+         end.
+
+    Definition complete_trace_prop (tr : Trace) : Prop
+       := protocol_trace_prop tr
+          /\
+          match tr with 
+          | Finite _ _ => terminating_trace_prop tr
+          | Infinite _ _ => True
           end.
 
-      Definition trace_first (tr : Trace) : state
-        :=
-          match tr with
-          | Finite s _ => s
-          | Infinite s _ => s
-          end.
-
-      Inductive Trace_messages : Type :=
-      | Finite_messages : list (option message) -> Trace_messages
-      | Infinite_messages : Stream (option message) -> Trace_messages. 
-
-      Definition protocol_output_messages_trace (tr : protocol_trace) : Trace_messages :=
-        match proj1_sig tr with
-        | Finite _ ls => Finite_messages (List.map output ls)
-        | Infinite _ st => Infinite_messages (map output st) end.
-
-      Definition protocol_input_messages_trace (tr : protocol_trace) : Trace_messages :=
-        match proj1_sig tr with
-        | Finite _ ls => Finite_messages (List.map input ls)
-        | Infinite _ st => Infinite_messages (map input st) end.
-
-      (* Defining equivocation on these trace definitions *)
-      (* Section 7 :
-  A message m received by a protocol state s with a transition label l in a
-  protocol execution trace is called "an equivocation" if it wasn't produced
-  in that trace
-       *)
-
-      Definition trace_prefix
-                 (tr : Trace)
-                 (last : in_state_out)
-                 (prefix : list in_state_out)
-        :=
-          match tr with
-          | Finite s ls => exists suffix, ls = prefix ++ (last :: suffix)
-          | Infinite s st => exists suffix, st = stream_app prefix (Cons last suffix)
-          end.
-
-      (** A finite trace is terminating if there's no other trace that contains it as a (proper) prefix.**)
-
-      Definition terminating_trace_prop (tr : Trace) : Prop 
-         :=
-           match tr with 
-           | Finite s ls => 
-               (exists (tr : protocol_trace) 
-               (last : in_state_out), 
-               trace_prefix (proj1_sig tr) last ls) -> False 
-           | Infinite s ls => False
-           end.
-
-      Definition complete_trace_prop (tr : Trace) : Prop
-         := ptrace_prop tr
-            /\
-            match tr with 
-            | Finite _ _ => terminating_trace_prop tr
-            | Infinite _ _ => True
-            end.
-
-      Lemma trace_prefix_protocol
-            (tr : protocol_trace)
-            (last : in_state_out)
-            (prefix : list in_state_out)
-            (Hprefix : trace_prefix (proj1_sig tr) last prefix)
-        : ptrace_prop (Finite (trace_first (proj1_sig tr)) (prefix ++ [last])).
-      Proof.
-        destruct tr as [tr Htr]. simpl in *.
-        generalize dependent tr. generalize dependent last.
-        apply (rev_ind (fun prefix => forall (last : in_state_out) (tr : Trace), ptrace_prop tr -> trace_prefix tr last prefix -> finite_ptrace (trace_first tr) (prefix ++ [last]))).
-        - intros last tr Htr Hprefix; destruct tr as [ | ]; unfold trace_prefix in Hprefix;   simpl in Hprefix
-          ; destruct Hprefix as [suffix Heq]; subst; destruct Htr as [Htr Hinit]
-          ; unfold trace_first; simpl; constructor; try assumption
-          ; inversion Htr; subst; clear Htr
-          ; specialize
-              (finite_ptrace_extend
-                 s1 [] (finite_ptrace_empty _ (protocol_transition_destination H3))
-                 s iom oom l1); intro Hext
-          ; apply Hext; assumption.
-        - intros last_p p Hind last tr Htr Hprefix.
-          specialize (Hind last_p tr Htr).
-          destruct tr as [ | ]; unfold trace_prefix in Hprefix;   simpl in Hprefix
-          ; destruct Hprefix as [suffix Heq]; subst; destruct Htr as [Htr Hinit]; simpl; simpl in Hind
-          ; split; try assumption
-          .
-          + assert
-              (Hex : exists suffix0 : list in_state_out,
-                  (p ++ [last_p]) ++ last :: suffix = p ++ last_p :: suffix0
-              ) by (exists (last :: suffix); rewrite <- app_assoc; reflexivity)
-            ; specialize (Hind Hex); clear Hex
-            ; destruct Hind as [Hptr _]
-            ; destruct last
-            ; apply extend_right_finite_trace_from
-            ; try assumption
-            .
-            rewrite <- (app_cons {| l := l1; input := input0; destination := destination0; output := output0 |} suffix) in Htr.
-            rewrite app_assoc in Htr. 
-            rewrite <- (app_assoc p _ _) in Htr. simpl in Htr.
-            rewrite <- app_assoc in Htr. 
-            specialize
-              (finite_ptrace_consecutive_valid_transition
-                 s
-                 (p ++ [last_p; {| l := l1; input := input0; destination := destination0; output := output0 |}] ++ suffix)
-                 suffix
-                 p
-                 last_p
-                 {| l := l1; input := input0; destination := destination0; output := output0 |}
-                 Htr
-                 eq_refl
-              ).
-            simpl.
-            rewrite map_app. simpl. rewrite last_is_last. tauto.
-          + assert
-              (Hex : exists suffix0 : Stream in_state_out,
-                  stream_app (p ++ [last_p])  (Cons last suffix) = stream_app p (Cons last_p suffix0)
-              ) by (exists (Cons last suffix); rewrite <- stream_app_assoc; reflexivity)
-            ; specialize (Hind Hex); clear Hex
-            ; destruct Hind as [Hptr _]
-            ; destruct last
-            ; apply extend_right_finite_trace_from
-            ; try assumption
-            .
-            rewrite <- stream_app_cons in Htr.
-            rewrite stream_app_assoc in Htr. 
-            rewrite <- (app_assoc p _ _) in Htr. simpl in Htr.
-            specialize
-              (infinite_ptrace_consecutive_valid_transition
-                 s
-                 (stream_app (p ++ [last_p; {| l := l1; input := input0; destination := destination0; output := output0 |}]) suffix)
-                 suffix
-                 p
-                 last_p
-                 {| l := l1; input := input0; destination := destination0; output := output0 |}
-                 Htr
-                 eq_refl
-              ).
-            simpl.
-            rewrite map_app. simpl. rewrite last_is_last. tauto.
-      Qed.
-
-      (* Implicitly, the state itself must be in the trace, and minimally the last element of the trace *)
-      (* Also implicitly, the trace leading up to the state is finite *)
-
-      Definition equivocation_in_trace
-                 (msg : message)
-                 (tr : protocol_trace)
-        : Prop
-        :=
-          exists (last : in_state_out),
-          exists (prefix : list in_state_out),
-            trace_prefix (proj1_sig tr) last prefix
-            /\  input last = Some msg
-            /\  ~ In (Some msg) (List.map output prefix)
-      .
-
-      Definition equivocation (msg : message) (s : state) : Prop :=
-        exists (tr : protocol_trace), trace_last (proj1_sig tr) = Some s /\ equivocation_in_trace msg tr.
-
-      (* Now we can have decidable equivocations! *) 
-      (* 6.2.1 Identifying equivocations *)
-      Definition has_been_sent (msg : message) (s : state) : Prop :=
-        forall (tr : protocol_trace) 
+    Lemma trace_prefix_protocol
+          (tr : protocol_trace)
           (last : in_state_out)
           (prefix : list in_state_out)
-          (Hpr : trace_prefix (proj1_sig tr) last prefix)
-          (Hlast : destination last = s),
-          List.Exists (fun (elem : in_state_out) => output elem = Some msg) prefix. 
+          (Hprefix : trace_prefix (proj1_sig tr) last prefix)
+      : protocol_trace_prop (Finite (trace_first (proj1_sig tr)) (prefix ++ [last])).
+    Proof.
+      destruct tr as [tr Htr]. simpl in *.
+      generalize dependent tr. generalize dependent last.
+      apply (rev_ind (fun prefix => forall (last : in_state_out) (tr : Trace), protocol_trace_prop tr -> trace_prefix tr last prefix -> finite_ptrace (trace_first tr) (prefix ++ [last]))).
+      - intros last tr Htr Hprefix; destruct tr as [ | ]; unfold trace_prefix in Hprefix;   simpl in Hprefix
+        ; destruct Hprefix as [suffix Heq]; subst; destruct Htr as [Htr Hinit]
+        ; unfold trace_first; simpl; constructor; try assumption
+        ; inversion Htr; subst; clear Htr
+        ; specialize
+            (finite_ptrace_extend
+               s1 [] (finite_ptrace_empty _ (protocol_transition_destination H3))
+               s iom oom l1); intro Hext
+        ; apply Hext; assumption.
+      - intros last_p p Hind last tr Htr Hprefix.
+        specialize (Hind last_p tr Htr).
+        destruct tr as [ | ]; unfold trace_prefix in Hprefix;   simpl in Hprefix
+        ; destruct Hprefix as [suffix Heq]; subst; destruct Htr as [Htr Hinit]; simpl; simpl in Hind
+        ; split; try assumption
+        .
+        + assert
+            (Hex : exists suffix0 : list in_state_out,
+                (p ++ [last_p]) ++ last :: suffix = p ++ last_p :: suffix0
+            ) by (exists (last :: suffix); rewrite <- app_assoc; reflexivity)
+          ; specialize (Hind Hex); clear Hex
+          ; destruct Hind as [Hptr _]
+          ; destruct last
+          ; apply extend_right_finite_trace_from
+          ; try assumption
+          .
+          rewrite <- (app_cons {| l := l1; input := input0; destination := destination0; output := output0 |} suffix) in Htr.
+          rewrite app_assoc in Htr. 
+          rewrite <- (app_assoc p _ _) in Htr. simpl in Htr.
+          rewrite <- app_assoc in Htr. 
+          specialize
+            (finite_ptrace_consecutive_valid_transition
+               s
+               (p ++ [last_p; {| l := l1; input := input0; destination := destination0; output := output0 |}] ++ suffix)
+               suffix
+               p
+               last_p
+               {| l := l1; input := input0; destination := destination0; output := output0 |}
+               Htr
+               eq_refl
+            ).
+          simpl.
+          rewrite map_app. simpl. rewrite last_is_last. tauto.
+        + assert
+            (Hex : exists suffix0 : Stream in_state_out,
+                stream_app (p ++ [last_p])  (Cons last suffix) = stream_app p (Cons last_p suffix0)
+            ) by (exists (Cons last suffix); rewrite <- stream_app_assoc; reflexivity)
+          ; specialize (Hind Hex); clear Hex
+          ; destruct Hind as [Hptr _]
+          ; destruct last
+          ; apply extend_right_finite_trace_from
+          ; try assumption
+          .
+          rewrite <- stream_app_cons in Htr.
+          rewrite stream_app_assoc in Htr. 
+          rewrite <- (app_assoc p _ _) in Htr. simpl in Htr.
+          specialize
+            (infinite_ptrace_consecutive_valid_transition
+               s
+               (stream_app (p ++ [last_p; {| l := l1; input := input0; destination := destination0; output := output0 |}]) suffix)
+               suffix
+               p
+               last_p
+               {| l := l1; input := input0; destination := destination0; output := output0 |}
+               Htr
+               eq_refl
+            ).
+          simpl.
+          rewrite map_app. simpl. rewrite last_is_last. tauto.
+    Qed.
 
-      (* Since equality of proto_messages is decidable, this function must exist : *) 
-      Definition proto_message_eqb {Eqd : EqDec message}
-                 (om1 : option message)
-                 (om2 : option message)
-        : bool
-        :=
-          match om1, om2 with
-          | None, None => true
-          | Some m1, Some m2 => if eq_dec m1 m2 then true else false
-          | _, _ => false
-          end.
+    (* Implicitly, the state itself must be in the trace, and minimally the last element of the trace *)
+    (* Also implicitly, the trace leading up to the state is finite *)
 
-      Fixpoint has_been_sentb
-               {Eqd : EqDec message}
-               (msg : message) (ls : list in_state_out) : bool
-        :=
-          existsb (fun x => proto_message_eqb (output x) (Some msg)) ls.
+    Definition equivocation_in_trace
+               (msg : message)
+               (tr : protocol_trace)
+      : Prop
+      :=
+        exists (last : in_state_out),
+        exists (prefix : list in_state_out),
+          trace_prefix (proj1_sig tr) last prefix
+          /\  input last = Some msg
+          /\  ~ In (Some msg) (List.map output prefix)
+    .
 
-      (* Now we can show that the above and below definitions are unnecessary *) 
+    Definition equivocation (msg : message) (s : state) : Prop :=
+      exists (tr : protocol_trace), trace_last (proj1_sig tr) = Some s /\ equivocation_in_trace msg tr.
 
-      (* Implicitly, the trace must be a protocol trace and also end with the state *) 
-      Definition finite_ptrace_upto 
-                 (s : state)
-                 (tr : protocol_trace)
-        : Prop
-        :=
-          trace_last (proj1_sig tr) = Some s
+    (* Now we can have decidable equivocations! *) 
+    (* 6.2.1 Identifying equivocations *)
+    Definition has_been_sent (msg : message) (s : state) : Prop :=
+      forall (tr : protocol_trace) 
+        (last : in_state_out)
+        (prefix : list in_state_out)
+        (Hpr : trace_prefix (proj1_sig tr) last prefix)
+        (Hlast : destination last = s),
+        List.Exists (fun (elem : in_state_out) => output elem = Some msg) prefix. 
+
+    (* Since equality of proto_messages is decidable, this function must exist : *) 
+    Definition proto_message_eqb {Eqd : EqDec message}
+               (om1 : option message)
+               (om2 : option message)
+      : bool
+      :=
+        match om1, om2 with
+        | None, None => true
+        | Some m1, Some m2 => if eq_dec m1 m2 then true else false
+        | _, _ => false
+        end.
+
+    Fixpoint has_been_sentb
+             {Eqd : EqDec message}
+             (msg : message) (ls : list in_state_out) : bool
+      :=
+        existsb (fun x => proto_message_eqb (output x) (Some msg)) ls.
+
+    (* Now we can show that the above and below definitions are unnecessary *) 
+
+    (* Implicitly, the trace must be a protocol trace and also end with the state *) 
+    Definition finite_ptrace_upto 
+               (s : state)
+               (tr : protocol_trace)
+      : Prop
+      :=
+        trace_last (proj1_sig tr) = Some s
+    .
+
+    (* 6.2.2 Equivocation-free as a composition constraint *)
+    Definition composition_constraint : Type :=
+      label -> state * option message -> Prop. 
+
+    Definition equivocation_free : composition_constraint :=
+      fun l som => match (snd som) with
+                | None => True
+                | Some msg => equivocation msg (fst som) -> False
+                end.
+
+    (* Decidable VLSMs *) 
+
+    Class VLSM_vdecidable :=
+      { valid_decidable : forall l som, {valid l som} + {~valid l som} 
+      }.
+
+  End VLSM.
+
+  Section VLSM_equality. (* Section 2.2.3 *)
+
+    Context
+      {message : Type}
+      {vtype : VLSM_type message}.
+
+    Definition VLSM_incl
+      {SigX SigY: LSM_sig vtype}
+      (X : VLSM SigX) (Y : VLSM SigY)
+      :=
+      forall t : Trace,
+        protocol_trace_prop X t -> protocol_trace_prop Y t
       .
 
-      (* 6.2.2 Equivocation-free as a composition constraint *)
-      Definition composition_constraint : Type :=
-        label -> state * option message -> Prop. 
+    Definition VLSM_eq
+      {SigX SigY: LSM_sig vtype}
+      (X : VLSM SigX) (Y : VLSM SigY)
+      :=
+      forall t : Trace,
+        protocol_trace_prop X t <-> protocol_trace_prop Y t
+      .
 
-      Definition equivocation_free : composition_constraint :=
-        fun l som => match (snd som) with
-                  | None => True
-                  | Some msg => equivocation msg (fst som) -> False
-                  end.
+    Lemma VLSM_eq_incl_l
+      {SigX SigY: LSM_sig vtype}
+      (X : VLSM SigX) (Y : VLSM SigY)
+      : VLSM_eq X Y -> VLSM_incl X Y 
+      .
+    Proof.
+      intro Heq.
+      intros t Hxt.
+      apply Heq.
+      assumption.
+    Qed.
+    
+    Lemma VLSM_eq_incl_r
+      {SigX SigY: LSM_sig vtype}
+      (X : VLSM SigX) (Y : VLSM SigY)
+      : VLSM_eq X Y -> VLSM_incl Y X 
+      .
+    Proof.
+      intro Heq.
+      intros t Hyt.
+      apply Heq.
+      assumption.
+    Qed.
 
-      (* Decidable VLSMs *) 
+    Lemma VLSM_eq_incl_iff
+      {SigX SigY: LSM_sig vtype}
+      (X : VLSM SigX) (Y : VLSM SigY)
+      : VLSM_eq X Y <-> VLSM_incl X Y /\ VLSM_incl Y X
+      .
+    Proof.
+      split.
+      - intro Heq.
+        split.
+        + apply VLSM_eq_incl_l; assumption.
+        + apply VLSM_eq_incl_r; assumption.
+      - intros [Hxy Hyx].
+        intro t.
+        split.
+        + apply Hxy.
+        + apply Hyx.
+    Qed.
 
-      Class VLSM_vdecidable :=
-        { valid_decidable : forall l som, {valid l som} + {~valid l som} 
-        }.
+  End VLSM_equality.
 
-    End VLSM.
+  Definition message_full_vlsm_sig
+    {message : Type}
+    {vtype : VLSM_type message}
+    {Sig : LSM_sig vtype}
+    (X : VLSM Sig)
+    : LSM_sig vtype
+    :=
+    {| initial_state_prop := @initial_state_prop _ _ Sig
+     ; initial_message_prop := fun message => True
+     ; s0 := @s0 _ _ Sig
+     ; m0 := @m0 _ _ Sig
+     ; l0 := @l0 _ _ Sig
+    |}.
 
-    Section VLSM_equality. (* Section 2.2.3 *)
+  Definition message_full_vlsm
+    {message : Type}
+    {vtype : VLSM_type message}
+    {Sig : LSM_sig vtype}
+    (X : VLSM Sig)
+    : VLSM (message_full_vlsm_sig X)
+    := 
+    {| transition := @transition _ _ _ X
+     ; valid := @valid _ _ _ X
+    |}.
 
-      Context
-        {message : Type}
-        {vtype : VLSM_type message}.
-      
-      Definition VLSM_eq
-        {SigX SigY: LSM_sig vtype}
-        (X : VLSM SigX) (Y : VLSM SigY)
-        :=
-        forall t : Trace_states,
-          protocol_state_trace_prop X t <-> protocol_state_trace_prop Y t
-        .
+  Lemma message_full_protocol_prop
+    {message : Type}
+    {vtype : VLSM_type message}
+    {Sig : LSM_sig vtype}
+    (X : VLSM Sig)
+    (s : state)
+    (om : option message)
+    (Hps : protocol_prop X (s, om))
+    : protocol_prop (message_full_vlsm X) (s, om).
+  Proof.
+    induction Hps.
+    - apply (protocol_initial_state (message_full_vlsm X) is).
+    - destruct im as [m Him]. simpl in om0. clear Him.
+      assert (Him : @initial_message_prop _ _ (message_full_vlsm_sig X) m)
+        by exact I.
+      apply (protocol_initial_message (message_full_vlsm X) (exist _ m Him)).
+    - apply (protocol_generated (message_full_vlsm X)) with _om _s; assumption.
+  Qed.
 
-    End VLSM_equality.
+  Lemma message_full_verbose_valid_protocol_transition
+    {message : Type}
+    {vtype : VLSM_type message}
+    {Sig : LSM_sig vtype}
+    (X : VLSM Sig)
+    (l : label)
+    (is os : state)
+    (iom oom : option message)
+    (Ht : verbose_valid_protocol_transition X l is os iom oom)
+    : verbose_valid_protocol_transition (message_full_vlsm X) l is os iom oom
+    .
+  Proof.
+    destruct Ht as [[_om Hps] [[_s Hpm] [Hv Ht]]].
+    repeat (split; try assumption).
+    - exists _om. apply message_full_protocol_prop. assumption.
+    - exists _s. apply message_full_protocol_prop. assumption.
+  Qed.
+
+  Lemma message_full_finite_ptrace
+    {message : Type}
+    {vtype : VLSM_type message}
+    {Sig : LSM_sig vtype}
+    (X : VLSM Sig)
+    (s : state)
+    (ls : list in_state_out)
+    (Hpxt : finite_ptrace_from X s ls)
+    : finite_ptrace_from (message_full_vlsm X) s ls
+    .
+  Proof.
+    induction Hpxt.
+    - constructor.
+      destruct H as [m H].
+      apply message_full_protocol_prop in H.
+      exists m. assumption.
+    - constructor; try assumption.
+      apply message_full_verbose_valid_protocol_transition. assumption.
+  Qed.
+
+  Lemma message_full_infinite_ptrace
+    {message : Type}
+    {vtype : VLSM_type message}
+    {Sig : LSM_sig vtype}
+    (X : VLSM Sig)
+    (s : state)
+    (ls : Stream in_state_out)
+    (Hpxt : infinite_ptrace_from X s ls)
+    : infinite_ptrace_from (message_full_vlsm X) s ls
+    .
+  Proof.
+    generalize dependent ls. generalize dependent s.
+    cofix H.
+    intros s [[l input destination output] ls] Hx.
+    inversion Hx; subst.
+    specialize (H destination ls H3).
+    constructor; try assumption.
+    apply message_full_verbose_valid_protocol_transition.
+    assumption.
+  Qed.
+
+  Lemma vlsm_incl_message_full_vlsm
+    {message : Type}
+    {vtype : VLSM_type message}
+    {Sig : LSM_sig vtype}
+    (X : VLSM Sig)
+    (Full := message_full_vlsm X)
+    : VLSM_incl X Full
+    .
+  Proof.
+    intros [s ls| s ss]; simpl; intros [Hxt Hinit].  
+    - apply message_full_finite_ptrace in Hxt.
+      split; try assumption.
+    - apply message_full_infinite_ptrace in Hxt.
+      split; try assumption.
+  Qed.
+
+  
